Prefix(:=<https://w3id.org/skgo/modsci#>)
Prefix(cc:=<http://creativecommons.org/ns#>)
Prefix(dc:=<http://purl.org/dc/elements/1.1/>)
Prefix(owl:=<http://www.w3.org/2002/07/owl#>)
Prefix(rdf:=<http://www.w3.org/1999/02/22-rdf-syntax-ns#>)
Prefix(xml:=<http://www.w3.org/XML/1998/namespace>)
Prefix(xsd:=<http://www.w3.org/2001/XMLSchema#>)
Prefix(foaf:=<http://xmlns.com/foaf/0.1/>)
Prefix(rdfs:=<http://www.w3.org/2000/01/rdf-schema#>)
Prefix(role:=<http://purl.obolibrary.org/obo/>)
Prefix(skos:=<http://www.w3.org/2004/02/skos/core#>)
Prefix(vann:=<http://purl.org/vocab/vann/>)
Prefix(sweet:=<http://sweetontology.net/phen/>)
Prefix(terms:=<http://purl.org/dc/terms/>)
Prefix(modsci:=<https://w3id.org/skgo/modsci#>)
Prefix(cpannotationschema:=<http://www.ontologydesignpatterns.org/schemas/cpannotationschema.owl#>)


Ontology(<https://w3id.org/skgo/modsci#>
<https://w3id.org/skgo/modsci/1.1>
Import(<http://www.w3.org/2004/02/skos/core>)
Annotation(dc:creator <https://orcid.org/0000-0002-2818-5890>)
Annotation(terms:contributor <https://orcid.org/0000-0001-9879-3827>)
Annotation(terms:contributor <https://orcid.org/0000-0002-0698-2864>)
Annotation(terms:description "ModSci is a reference ontology for modelling different types of modern sciences and related entities, such as scientific discoveries, renowned scientists, instruments, phenomena ... etc."@en)
Annotation(terms:license <http://creativecommons.org/licenses/by/3.0/>)
Annotation(terms:modified "2022-12-18")
Annotation(terms:title "ModSci, Modern Science Ontology."@en)
Annotation(vann:preferredNamespacePrefix "modsci")
Annotation(owl:versionInfo "1.1"^^xsd:decimal)

Declaration(Class(sweet:Phenomenon))
Declaration(Class(rdf:List))
Declaration(Class(foaf:Organization))
Declaration(Class(foaf:Person))
Declaration(Class(modsci:AcidbaseChemistry))
Declaration(Class(modsci:Acoustics))
Declaration(Class(modsci:Agriculture))
Declaration(Class(modsci:Agronomy))
Declaration(Class(modsci:Algebra))
Declaration(Class(modsci:Algorithms))
Declaration(Class(modsci:AnalyticalChemistry))
Declaration(Class(modsci:AnalyticalSpectrometry))
Declaration(Class(modsci:Anatomy))
Declaration(Class(modsci:AnimalProduction))
Declaration(Class(modsci:Anthropology))
Declaration(Class(modsci:ApplicationOfScience))
Declaration(Class(modsci:AppliedMathematics))
Declaration(Class(modsci:AppliedMechanics))
Declaration(Class(modsci:AppliedPhysics))
Declaration(Class(modsci:AppliedSciences))
Declaration(Class(modsci:ApproximationTheory))
Declaration(Class(modsci:Archaeology))
Declaration(Class(modsci:Architecture))
Declaration(Class(modsci:ArtificialIntelligence))
Declaration(Class(modsci:Astrobiology))
Declaration(Class(modsci:Astrochemistry))
Declaration(Class(modsci:Astrometry))
Declaration(Class(modsci:AstronomicalPhenomena))
Declaration(Class(modsci:Astronomy))
Declaration(Class(modsci:AtmosphericPhenomena))
Declaration(Class(modsci:AtmosphericSciences))
Declaration(Class(modsci:AtomicPhysics))
Declaration(Class(modsci:AutomataTheory))
Declaration(Class(modsci:AutomatedReasoning))
Declaration(Class(modsci:BasinAnalysis))
Declaration(Class(modsci:BehaviouralSciences))
Declaration(Class(modsci:Biochemistry))
Declaration(Class(modsci:Bioengineering))
Declaration(Class(modsci:Bioethics))
Declaration(Class(modsci:Biogeography))
Declaration(Class(modsci:Bioinformatics))
Declaration(Class(modsci:BioinformaticsSoftware))
Declaration(Class(modsci:BioinorganicChemistry))
Declaration(Class(modsci:BiologicalMathematics))
Declaration(Class(modsci:BiologicalOceanography))
Declaration(Class(modsci:BiologicalPhenomena))
Declaration(Class(modsci:Biology))
Declaration(Class(modsci:BiomedicalEngineering))
Declaration(Class(modsci:Biophysics))
Declaration(Class(modsci:Biopsychology))
Declaration(Class(modsci:Biostatistics))
Declaration(Class(modsci:Biotechnology))
Declaration(Class(modsci:Botany))
Declaration(Class(modsci:CalculusOfVariations))
Declaration(Class(modsci:Catalysis))
Declaration(Class(modsci:CellBiology))
Declaration(Class(modsci:ChemicalCharacterisationOfMaterials))
Declaration(Class(modsci:ChemicalEngineering))
Declaration(Class(modsci:ChemicalOceanography))
Declaration(Class(modsci:ChemicalPhenomena))
Declaration(Class(modsci:ChemicalThermodynamics))
Declaration(Class(modsci:Chemistry))
Declaration(Class(modsci:ClassicalPhysics))
Declaration(Class(modsci:ClassificationAlgorithms))
Declaration(Class(modsci:CoalGeology))
Declaration(Class(modsci:CodingAndInformationTheory))
Declaration(Class(modsci:CognitiveScience))
Declaration(Class(modsci:Colloid))
Declaration(Class(modsci:ColloidalChemistry))
Declaration(Class(modsci:CommunicationAndSecurity))
Declaration(Class(modsci:CommunicationStudies))
Declaration(Class(modsci:CompilerTheory))
Declaration(Class(modsci:ComputabilityTheory))
Declaration(Class(modsci:ComputationalComplexityTheory))
Declaration(Class(modsci:ComputationalLinguistics))
Declaration(Class(modsci:ComputationalMathematics))
Declaration(Class(modsci:ComputationalPhysics))
Declaration(Class(modsci:Computer-HumanInteraction))
Declaration(Class(modsci:ComputerApplications))
Declaration(Class(modsci:ComputerConcurrency))
Declaration(Class(modsci:ComputerGraphics))
Declaration(Class(modsci:ComputerScience))
Declaration(Class(modsci:ComputerSecurity))
Declaration(Class(modsci:ComputerSoftware))
Declaration(Class(modsci:ComputerSystemArchitecture))
Declaration(Class(modsci:ComputerVision))
Declaration(Class(modsci:ConceptualModelling))
Declaration(Class(modsci:CondensedMatterPhysics))
Declaration(Class(modsci:Cosmology))
Declaration(Class(modsci:CropProduction))
Declaration(Class(modsci:Cryobiology))
Declaration(Class(modsci:Cryptography))
Declaration(Class(modsci:Crystallography))
Declaration(Class(modsci:CulturalStudies))
Declaration(Class(modsci:Cybernetics))
Declaration(Class(modsci:DataEncryption))
Declaration(Class(modsci:DataFormat))
Declaration(Class(modsci:DataMining))
Declaration(Class(modsci:DataStructures))
Declaration(Class(modsci:DatabaseManagement))
Declaration(Class(modsci:DecisionSupportSystems))
Declaration(Class(modsci:Dentistry))
Declaration(Class(modsci:DevelopmentalBiology))
Declaration(Class(modsci:DifferentialEquations))
Declaration(Class(modsci:DiscoveryOfMethods))
Declaration(Class(modsci:DiscoveryOfPhenomenon))
Declaration(Class(modsci:DiscreteMathematics))
Declaration(Class(modsci:DistributedComputing))
Declaration(Class(modsci:DistributedSystems))
Declaration(Class(modsci:EarthScience))
Declaration(Class(modsci:EcologicalApplications))
Declaration(Class(modsci:Ecology))
Declaration(Class(modsci:Economics))
Declaration(Class(modsci:Education))
Declaration(Class(modsci:ElectroanalyticalChemistry))
Declaration(Class(modsci:Electrochemistry))
Declaration(Class(modsci:Electrodynamics))
Declaration(Class(modsci:Electrostatics))
Declaration(Class(modsci:Engineering))
Declaration(Class(modsci:EnvironmentalChemistry))
Declaration(Class(modsci:EnvironmentalScience))
Declaration(Class(modsci:Epidemiology))
Declaration(Class(modsci:Ergonomics))
Declaration(Class(modsci:EthnicStudies))
Declaration(Class(modsci:Ethnobiology))
Declaration(Class(modsci:Ethnology))
Declaration(Class(modsci:Ethology))
Declaration(Class(modsci:EvolutionaryBiology))
Declaration(Class(modsci:EvolutionaryComputation))
Declaration(Class(modsci:EvolutionaryPsychology))
Declaration(Class(modsci:ExperimentalPhysics))
Declaration(Class(modsci:ExtragalacticAstronomy))
Declaration(Class(modsci:ExtraterrestrialGeology))
Declaration(Class(modsci:FinancialMathematics))
Declaration(Class(modsci:FisheriesSciences))
Declaration(Class(modsci:FlowAnalysis))
Declaration(Class(modsci:FluidPhysics))
Declaration(Class(modsci:FoodChemistry))
Declaration(Class(modsci:Forensics))
Declaration(Class(modsci:Forestry))
Declaration(Class(modsci:ForestrySciences))
Declaration(Class(modsci:FormalScience))
Declaration(Class(modsci:FreeRadicalChemistry))
Declaration(Class(modsci:FunctionalAnalysis))
Declaration(Class(modsci:GalacticAstronomy))
Declaration(Class(modsci:Genetics))
Declaration(Class(modsci:Geochemistry))
Declaration(Class(modsci:Geochronology))
Declaration(Class(modsci:Geodesy))
Declaration(Class(modsci:Geodynamics))
Declaration(Class(modsci:Geography))
Declaration(Class(modsci:GeologicalPhenomena))
Declaration(Class(modsci:GeologicalSciences))
Declaration(Class(modsci:Geology))
Declaration(Class(modsci:Geomorphology))
Declaration(Class(modsci:GeophysicalFluidDynamics))
Declaration(Class(modsci:Geophysics))
Declaration(Class(modsci:Geothermics))
Declaration(Class(modsci:Gerontology))
Declaration(Class(modsci:Glaciology))
Declaration(Class(modsci:GlobalInformationSystems))
Declaration(Class(modsci:Gravimetrics))
Declaration(Class(modsci:GreenChemistry))
Declaration(Class(modsci:Health))
Declaration(Class(modsci:HealthSciences))
Declaration(Class(modsci:Healthcare))
Declaration(Class(modsci:History))
Declaration(Class(modsci:HomologicalAlgebra))
Declaration(Class(modsci:HorticulturalProduction))
Declaration(Class(modsci:HumanComputerInteraction))
Declaration(Class(modsci:HumanSciences))
Declaration(Class(modsci:Hydrology))
Declaration(Class(modsci:ImageProcessing))
Declaration(Class(modsci:Immunology))
Declaration(Class(modsci:IndustrialScience))
Declaration(Class(modsci:Industry))
Declaration(Class(modsci:InformationRetrieval))
Declaration(Class(modsci:InformationScience))
Declaration(Class(modsci:InformationSystems))
Declaration(Class(modsci:InformationSystemsManagement))
Declaration(Class(modsci:InformationSystemsTheory))
Declaration(Class(modsci:InformationVisualization))
Declaration(Class(modsci:Informetrics))
Declaration(Class(modsci:InorganicChemistry))
Declaration(Class(modsci:InorganicGreenChemistry))
Declaration(Class(modsci:Instrument))
Declaration(Class(modsci:IntegralEquations))
Declaration(Class(modsci:InterdisciplinaryStudies))
Declaration(Class(modsci:InterorganisationalInformationSystems))
Declaration(Class(modsci:KnowledgeSystems))
Declaration(Class(modsci:LaboratoryInstrument))
Declaration(Class(modsci:Lasers))
Declaration(Class(modsci:LibraryScience))
Declaration(Class(modsci:Limnology))
Declaration(Class(modsci:Linguistics))
Declaration(Class(modsci:Logic))
Declaration(Class(modsci:MachineLearning))
Declaration(Class(modsci:Magnetism))
Declaration(Class(modsci:MainGroupMetalChemistry))
Declaration(Class(modsci:MarineBiology))
Declaration(Class(modsci:MarkupLanguages))
Declaration(Class(modsci:MaterialsChemistry))
Declaration(Class(modsci:MathematicalAndTheoreticalBiology))
Declaration(Class(modsci:MathematicalLogic))
Declaration(Class(modsci:MathematicalPhysics))
Declaration(Class(modsci:Mathematics))
Declaration(Class(modsci:Measurement))
Declaration(Class(modsci:Mechanics))
Declaration(Class(modsci:MechanismsOfReactions))
Declaration(Class(modsci:MedicinalChemistry))
Declaration(Class(modsci:Medicine))
Declaration(Class(modsci:Metabolism))
Declaration(Class(modsci:Metallurgy))
Declaration(Class(modsci:MetamorphicPetrology))
Declaration(Class(modsci:MeteorologicalPhenomena))
Declaration(Class(modsci:MetrologicalChemistry))
Declaration(Class(modsci:Metrology))
Declaration(Class(modsci:MilitaryScience))
Declaration(Class(modsci:Mineralogy))
Declaration(Class(modsci:MobileTechnologies))
Declaration(Class(modsci:ModernScience))
Declaration(Class(modsci:MolecularBiology))
Declaration(Class(modsci:MolecularPhysics))
Declaration(Class(modsci:MultimediaProgramming))
Declaration(Class(modsci:Museology))
Declaration(Class(modsci:Nanochemistry))
Declaration(Class(modsci:NaturalLanguageProcessing))
Declaration(Class(modsci:NaturalPhenomenon))
Declaration(Class(modsci:NaturalProductsChemistry))
Declaration(Class(modsci:NaturalScience))
Declaration(Class(modsci:Networking))
Declaration(Class(modsci:NeuralEngineering))
Declaration(Class(modsci:Neuroscience))
Declaration(Class(modsci:Non-equilibriumProcesses))
Declaration(Class(modsci:Non-metalChemistry))
Declaration(Class(modsci:NonlinearOptics))
Declaration(Class(modsci:NuclearChemistry))
Declaration(Class(modsci:NuclearPhysics))
Declaration(Class(modsci:NumberTheory))
Declaration(Class(modsci:NumericalAnalysis))
Declaration(Class(modsci:Nursing))
Declaration(Class(modsci:OceanographicPhenomena))
Declaration(Class(modsci:Oceanography))
Declaration(Class(modsci:OperatingSystems))
Declaration(Class(modsci:OperationsResearch))
Declaration(Class(modsci:OpticalCommunications))
Declaration(Class(modsci:OpticalPhysics))
Declaration(Class(modsci:Optics))
Declaration(Class(modsci:Optimisation))
Declaration(Class(modsci:Optoelectronics))
Declaration(Class(modsci:OrdinaryDifferentialEquations))
Declaration(Class(modsci:OreDepositPetrology))
Declaration(Class(modsci:OrganicChemicalSynthesis))
Declaration(Class(modsci:OrganicChemistry))
Declaration(Class(modsci:OrganicGreenChemistry))
Declaration(Class(modsci:OrganometallicChemistry))
Declaration(Class(modsci:Palaeomagnetism))
Declaration(Class(modsci:Palaeontology))
Declaration(Class(modsci:Paleoclimatology))
Declaration(Class(modsci:Paleontology))
Declaration(Class(modsci:Palynology))
Declaration(Class(modsci:ParallelComputing))
Declaration(Class(modsci:Parasitology))
Declaration(Class(modsci:PartialDifferentialEquations))
Declaration(Class(modsci:ParticlePhysics))
Declaration(Class(modsci:PastureProduction))
Declaration(Class(modsci:PatternRecognition))
Declaration(Class(modsci:PetroleumGeology))
Declaration(Class(modsci:Pharmacology))
Declaration(Class(modsci:Pharmacy))
Declaration(Class(modsci:Philosophy))
Declaration(Class(modsci:Photochemistry))
Declaration(Class(modsci:Photonics))
Declaration(Class(modsci:Phylogeny))
Declaration(Class(modsci:PhysicalChemistry))
Declaration(Class(modsci:PhysicalGeography))
Declaration(Class(modsci:PhysicalOceanography))
Declaration(Class(modsci:PhysicalOrganicChemistry))
Declaration(Class(modsci:PhysicalPhenomena))
Declaration(Class(modsci:Physics))
Declaration(Class(modsci:Physiology))
Declaration(Class(modsci:PlanetaryScience))
Declaration(Class(modsci:PlasmaPhysics))
Declaration(Class(modsci:PoliticalEconomy))
Declaration(Class(modsci:PoliticalScience))
Declaration(Class(modsci:PolymerisationMechanisms))
Declaration(Class(modsci:ProgrammingLanguage))
Declaration(Class(modsci:ProgrammingLanguageTheory))
Declaration(Class(modsci:ProgrammingLanguages))
Declaration(Class(modsci:Psychology))
Declaration(Class(modsci:PureMathematics))
Declaration(Class(modsci:QuantumComputing))
Declaration(Class(modsci:QuantumMechanics))
Declaration(Class(modsci:QuantumOptics))
Declaration(Class(modsci:QuantumPhysics))
Declaration(Class(modsci:Radiobiology))
Declaration(Class(modsci:Radiochemistry))
Declaration(Class(modsci:Radiometrics))
Declaration(Class(modsci:RelationalDatabases))
Declaration(Class(modsci:ReverseEngineering))
Declaration(Class(modsci:Robotics))
Declaration(Class(modsci:ScienceAndTechnologyStudies))
Declaration(Class(modsci:ScienceStudies))
Declaration(Class(modsci:ScientificDiscovery))
Declaration(Class(modsci:ScientificInstrument))
Declaration(Class(modsci:ScientificInstrumentManufacturer))
Declaration(Class(modsci:ScientificMethod))
Declaration(Class(modsci:ScientificModeling))
Declaration(Class(modsci:ScientificOrganization))
Declaration(Class(modsci:Scientist))
Declaration(Class(modsci:Sedimentology))
Declaration(Class(modsci:SeismicExploration))
Declaration(Class(modsci:Seismology))
Declaration(Class(modsci:Semantics))
Declaration(Class(modsci:Semiotics))
Declaration(Class(modsci:SeparationScience))
Declaration(Class(modsci:SocialPhenomenon))
Declaration(Class(modsci:SocialPsychology))
Declaration(Class(modsci:SocialSciences))
Declaration(Class(modsci:SocialWork))
Declaration(Class(modsci:Sociobiology))
Declaration(Class(modsci:Sociology))
Declaration(Class(modsci:SoftComputing))
Declaration(Class(modsci:SoftwareEngineering))
Declaration(Class(modsci:SoilBiology))
Declaration(Class(modsci:SoilScience))
Declaration(Class(modsci:SoilSciences))
Declaration(Class(modsci:SolidMechanics))
Declaration(Class(modsci:SolidStateChemistry))
Declaration(Class(modsci:SolutionChemistry))
Declaration(Class(modsci:SpaceScience))
Declaration(Class(modsci:Spectroscopy))
Declaration(Class(modsci:SportsScience))
Declaration(Class(modsci:Statistics))
Declaration(Class(modsci:StellarAstronomy))
Declaration(Class(modsci:Stereochemistry))
Declaration(Class(modsci:Stratigraphy))
Declaration(Class(modsci:StructuralChemistry))
Declaration(Class(modsci:StructuralGeology))
Declaration(Class(modsci:StructuredStorage))
Declaration(Class(modsci:SupramolecularChemistry))
Declaration(Class(modsci:SurfaceChemistry))
Declaration(Class(modsci:SynthesisOfMaterials))
Declaration(Class(modsci:SystemsScience))
Declaration(Class(modsci:Technology))
Declaration(Class(modsci:Tectonics))
Declaration(Class(modsci:TheoreticalBiology))
Declaration(Class(modsci:TheoreticalChemistry))
Declaration(Class(modsci:TheoreticalComputerScience))
Declaration(Class(modsci:TheoreticalLinguistics))
Declaration(Class(modsci:TheoryAndDesignOfMaterials))
Declaration(Class(modsci:TheoryOfComputation))
Declaration(Class(modsci:Thermodynamics))
Declaration(Class(modsci:Topology))
Declaration(Class(modsci:Toxicology))
Declaration(Class(modsci:Transdisciplinarity))
Declaration(Class(modsci:TransitionMetalChemistry))
Declaration(Class(modsci:TypeTheory))
Declaration(Class(modsci:UbiquitousComputing))
Declaration(Class(modsci:UniversalAlgebra))
Declaration(Class(modsci:UrbanPlanning))
Declaration(Class(modsci:VeterinaryMedicine))
Declaration(Class(modsci:VeterinarySciences))
Declaration(Class(modsci:VirtualReality))
Declaration(Class(modsci:Volcanology))
Declaration(Class(modsci:Waves))
Declaration(Class(modsci:WebSearch))
Declaration(Class(modsci:WebServices))
Declaration(Class(modsci:WebTechnologies))
Declaration(Class(modsci:Zoology))
Declaration(Class(modsci:f-BlockChemistry))
Declaration(ObjectProperty(modsci:appliesLawsFrom))
Declaration(ObjectProperty(modsci:appliesLawsFromMathematics))
Declaration(ObjectProperty(modsci:appliesLawsFromPhysics))
Declaration(ObjectProperty(modsci:appliesLawsFromStatistics))
Declaration(ObjectProperty(modsci:appliesLawsFromThermodynamics))
Declaration(ObjectProperty(modsci:discoveredByAppliedSciences))
Declaration(ObjectProperty(modsci:discoveredByBehaviouralSciences))
Declaration(ObjectProperty(modsci:discoveredByFormalScience))
Declaration(ObjectProperty(modsci:discoveredByHealthSciences))
Declaration(ObjectProperty(modsci:discoveredByInterdisciplinaryStudies))
Declaration(ObjectProperty(modsci:discoveredByMachine))
Declaration(ObjectProperty(modsci:discoveredByNaturalScience))
Declaration(ObjectProperty(modsci:discoveredByScience))
Declaration(ObjectProperty(modsci:discoveredByScientist))
Declaration(ObjectProperty(modsci:discoveredBySocialSciences))
Declaration(ObjectProperty(modsci:followsMethod))
Declaration(ObjectProperty(modsci:hasApplication))
Declaration(ObjectProperty(modsci:hasCloseRelationshipTo))
Declaration(ObjectProperty(modsci:hasCollaborationWith))
Declaration(ObjectProperty(modsci:hasManufacturer))
Declaration(ObjectProperty(modsci:hasMethodsInspiredFrom))
Declaration(ObjectProperty(modsci:hasScientificInstrumentManufacturer))
Declaration(ObjectProperty(modsci:inspiredFrom))
Declaration(ObjectProperty(modsci:inspiredFromPhenomenon))
Declaration(ObjectProperty(modsci:inspiredFromScientificDiscovery))
Declaration(ObjectProperty(modsci:instrumentInventedBy))
Declaration(ObjectProperty(modsci:instrumentUsedInScience))
Declaration(ObjectProperty(modsci:interestedInPhenomenon))
Declaration(ObjectProperty(modsci:isApplicationOfAppliedScience))
Declaration(ObjectProperty(modsci:isApplicationOfBehaviouralSciences))
Declaration(ObjectProperty(modsci:isApplicationOfFormalScience))
Declaration(ObjectProperty(modsci:isApplicationOfHealthSciences))
Declaration(ObjectProperty(modsci:isApplicationOfInterdisciplinaryStudies))
Declaration(ObjectProperty(modsci:isApplicationOfNaturalScience))
Declaration(ObjectProperty(modsci:isApplicationOfScience))
Declaration(ObjectProperty(modsci:isApplicationOfSocialSciences))
Declaration(ObjectProperty(modsci:isDiscoveredBy))
Declaration(ObjectProperty(modsci:isDiscoveredByOrganization))
Declaration(ObjectProperty(modsci:isDiscoveredByScientist))
Declaration(ObjectProperty(modsci:isManufacturerOf))
Declaration(ObjectProperty(modsci:isStudentOf))
Declaration(ObjectProperty(modsci:requiresKnowledgeFrom))
Declaration(ObjectProperty(modsci:scientistBelongsTo))
Declaration(ObjectProperty(modsci:suppliesSubstancesTo))
Declaration(ObjectProperty(modsci:takeSunstancesFrom))
Declaration(ObjectProperty(modsci:undertakesResearch))
Declaration(ObjectProperty(modsci:usesMethodsFrom))
Declaration(ObjectProperty(modsci:usesTechniquesFrom))
Declaration(DataProperty(modsci:InstrumentFunctionDesription))
Declaration(NamedIndividual(modsci:ADInstruments))
Declaration(NamedIndividual(modsci:Accelerometer))
Declaration(NamedIndividual(modsci:Accumulator))
Declaration(NamedIndividual(modsci:AgilentTechnologies))
Declaration(NamedIndividual(modsci:Ammeter))
Declaration(NamedIndividual(modsci:Anemometer))
Declaration(NamedIndividual(modsci:AntonPaar))
Declaration(NamedIndividual(modsci:Astronomical_Studies))
Declaration(NamedIndividual(modsci:Aurora))
Declaration(NamedIndividual(modsci:Barometer))
Declaration(NamedIndividual(modsci:Biochip))
Declaration(NamedIndividual(modsci:Biological_Studies))
Declaration(NamedIndividual(modsci:Biomedical_Signals))
Declaration(NamedIndividual(modsci:Biosensors))
Declaration(NamedIndividual(modsci:Boiling))
Declaration(NamedIndividual(modsci:Breaking_waves))
Declaration(NamedIndividual(modsci:Bruker))
Declaration(NamedIndividual(modsci:Caliper))
Declaration(NamedIndividual(modsci:Calorimeter))
Declaration(NamedIndividual(modsci:Chemical_Studies))
Declaration(NamedIndividual(modsci:Community_of_European_Solar_Radio_Astronomers))
Declaration(NamedIndividual(modsci:Conservation_of_energy))
Declaration(NamedIndividual(modsci:Crystal_growth))
Declaration(NamedIndividual(modsci:DNA_Sequencer))
Declaration(NamedIndividual(modsci:Decision_Trees))
Declaration(NamedIndividual(modsci:Decomposition))
Declaration(NamedIndividual(modsci:Deep_Learning))
Declaration(NamedIndividual(modsci:Dynamo))
Declaration(NamedIndividual(modsci:Dynamometer))
Declaration(NamedIndividual(modsci:E3G))
Declaration(NamedIndividual(modsci:EACSL))
Declaration(NamedIndividual(modsci:Earthquake))
Declaration(NamedIndividual(modsci:Economic_Studies))
Declaration(NamedIndividual(modsci:Electrometer))
Declaration(NamedIndividual(modsci:Electroscope))
Declaration(NamedIndividual(modsci:Elementar))
Declaration(NamedIndividual(modsci:Ellipsometer))
Declaration(NamedIndividual(modsci:Engineering_Studies))
Declaration(NamedIndividual(modsci:Erosion))
Declaration(NamedIndividual(modsci:Eudiometer))
Declaration(NamedIndividual(modsci:Evangelista_Torricelli))
Declaration(NamedIndividual(modsci:Fire))
Declaration(NamedIndividual(modsci:Fraunhofer))
Declaration(NamedIndividual(modsci:Freezing))
Declaration(NamedIndividual(modsci:Friedrich_Drexler))
Declaration(NamedIndividual(modsci:Galileo))
Declaration(NamedIndividual(modsci:Galvanometer))
Declaration(NamedIndividual(modsci:Genetic_algorithms))
Declaration(NamedIndividual(modsci:Geological_Studies))
Declaration(NamedIndividual(modsci:Gravitometer))
Declaration(NamedIndividual(modsci:Gravity))
Declaration(NamedIndividual(modsci:Growth))
Declaration(NamedIndividual(modsci:Guglielmo_Marconi))
Declaration(NamedIndividual(modsci:Haze))
Declaration(NamedIndividual(modsci:Historical_Studies))
Declaration(NamedIndividual(modsci:Horiba))
Declaration(NamedIndividual(modsci:Hydrometer))
Declaration(NamedIndividual(modsci:Inclinometer))
Declaration(NamedIndividual(modsci:Interferometer))
Declaration(NamedIndividual(modsci:Isaac_Newton))
Declaration(NamedIndividual(modsci:Johann_Schweigger))
Declaration(NamedIndividual(modsci:Julius_von_Mayer))
Declaration(NamedIndividual(modsci:KNN_Algorithm))
Declaration(NamedIndividual(modsci:LECO_Corporation))
Declaration(NamedIndividual(modsci:Light_Bulb))
Declaration(NamedIndividual(modsci:Light_magnification))
Declaration(NamedIndividual(modsci:Light_pillar))
Declaration(NamedIndividual(modsci:Linear_Regression))
Declaration(NamedIndividual(modsci:Magnetograph))
Declaration(NamedIndividual(modsci:Magnetometer))
Declaration(NamedIndividual(modsci:MalvernInstruments))
Declaration(NamedIndividual(modsci:Manometer))
Declaration(NamedIndividual(modsci:MarkesInternational))
Declaration(NamedIndividual(modsci:Mathematical_Studies))
Declaration(NamedIndividual(modsci:McPhersonInc))
Declaration(NamedIndividual(modsci:Metabolism))
Declaration(NamedIndividual(modsci:Michael_Faraday))
Declaration(NamedIndividual(modsci:Micrometer))
Declaration(NamedIndividual(modsci:Microscope))
Declaration(NamedIndividual(modsci:Movie_camera))
Declaration(NamedIndividual(modsci:NASA))
Declaration(NamedIndividual(modsci:NovacamTechnologies))
Declaration(NamedIndividual(modsci:Ocean_currents))
Declaration(NamedIndividual(modsci:Ohmmeter))
Declaration(NamedIndividual(modsci:Olaus_Roemer))
Declaration(NamedIndividual(modsci:OpenAI_Inc))
Declaration(NamedIndividual(modsci:Oscilloscope))
Declaration(NamedIndividual(modsci:Overpopulation))
Declaration(NamedIndividual(modsci:OxfordInstruments))
Declaration(NamedIndividual(modsci:PallCorp))
Declaration(NamedIndividual(modsci:Phonograph))
Declaration(NamedIndividual(modsci:Physical_Studies))
Declaration(NamedIndividual(modsci:PolymerChar))
Declaration(NamedIndividual(modsci:Population_decrease))
Declaration(NamedIndividual(modsci:PsychiatricDrugs))
Declaration(NamedIndividual(modsci:Psychological_Studies))
Declaration(NamedIndividual(modsci:Racism))
Declaration(NamedIndividual(modsci:Radio_Signals))
Declaration(NamedIndividual(modsci:Rainbow))
Declaration(NamedIndividual(modsci:Resampling_Methods))
Declaration(NamedIndividual(modsci:Rusting))
Declaration(NamedIndividual(modsci:Seismometer))
Declaration(NamedIndividual(modsci:ShimadzuCorp))
Declaration(NamedIndividual(modsci:Shrinkage))
Declaration(NamedIndividual(modsci:Spectrogram))
Declaration(NamedIndividual(modsci:Spectrometer))
Declaration(NamedIndividual(modsci:Speed_of_light))
Declaration(NamedIndividual(modsci:Statistics_Studies))
Declaration(NamedIndividual(modsci:Storm))
Declaration(NamedIndividual(modsci:Studying_biochemical_reactions))
Declaration(NamedIndividual(modsci:Subset_Selection))
Declaration(NamedIndividual(modsci:Subsun))
Declaration(NamedIndividual(modsci:Supernova))
Declaration(NamedIndividual(modsci:Support_Vector_Machines))
Declaration(NamedIndividual(modsci:Techtron))
Declaration(NamedIndividual(modsci:Telescope))
Declaration(NamedIndividual(modsci:The_Bridges_Organization))
Declaration(NamedIndividual(modsci:The_Fibonacci_Association))
Declaration(NamedIndividual(modsci:Theodolite))
Declaration(NamedIndividual(modsci:Thermocouple))
Declaration(NamedIndividual(modsci:Thermometer))
Declaration(NamedIndividual(modsci:Thomas_Edison))
Declaration(NamedIndividual(modsci:Time_Series_Analysis))
Declaration(NamedIndividual(modsci:Tsunamis))
Declaration(NamedIndividual(modsci:Volcano))
Declaration(NamedIndividual(modsci:Voltmeter))
Declaration(NamedIndividual(modsci:Waldemar_Jungner))
Declaration(NamedIndividual(modsci:WatersCorporation))
Declaration(NamedIndividual(modsci:Weddings))
Declaration(NamedIndividual(modsci:study_of_wetlands))
Declaration(NamedIndividual(modsci:temperature_gradient))
Declaration(AnnotationProperty(dc:creator))
Declaration(AnnotationProperty(dc:date))
Declaration(AnnotationProperty(terms:bibliographicCitation))
Declaration(AnnotationProperty(terms:contributor))
Declaration(AnnotationProperty(terms:created))
Declaration(AnnotationProperty(terms:creator))
Declaration(AnnotationProperty(terms:date))
Declaration(AnnotationProperty(terms:description))
Declaration(AnnotationProperty(terms:license))
Declaration(AnnotationProperty(terms:modified))
Declaration(AnnotationProperty(terms:title))
Declaration(AnnotationProperty(vann:preferredNamespacePrefix))
Declaration(AnnotationProperty(<http://swrl.stanford.edu/ontologies/3.3/swrla.owl#isRuleEnabled>))
Declaration(AnnotationProperty(skos:nationality))
Declaration(AnnotationProperty(skos:prefLabel))
Declaration(AnnotationProperty(foaf:familyName))
############################
#   Annotation Properties
############################

# Annotation Property: terms:date (Date)

AnnotationAssertion(terms:bibliographicCitation terms:date "[W3CDTF] http://www.w3.org/TR/NOTE-datetime")
AnnotationAssertion(rdfs:comment terms:date "Date may be used to express temporal information at any level of granularity. Recommended best practice is to use an encoding scheme, such as the W3CDTF profile of ISO 8601 [W3CDTF]."@en-us)
AnnotationAssertion(rdfs:label terms:date "Date"@en-us)
AnnotationAssertion(rdfs:seeAlso terms:date <http://www.w3.org/TR/NOTE-datetime>)
AnnotationAssertion(skos:definition terms:date "A point or period of time associated with an event in the lifecycle of the resource."@en-us)
SubAnnotationPropertyOf(terms:date dc:date)
AnnotationPropertyRange(terms:date rdfs:Literal)

# Annotation Property: terms:modified (Date Modified)

AnnotationAssertion(rdfs:label terms:modified "Date Modified"@en-us)
AnnotationAssertion(skos:definition terms:modified "Date on which the resource was changed."@en-us)
SubAnnotationPropertyOf(terms:modified terms:date)
AnnotationPropertyRange(terms:modified rdfs:Literal)

# Annotation Property: skos:nationality (skos:nationality)

SubAnnotationPropertyOf(skos:nationality rdfs:comment)


############################
#   Object Properties
############################

# Object Property: modsci:appliesLawsFrom (modsci:appliesLawsFrom)

AsymmetricObjectProperty(modsci:appliesLawsFrom)
ObjectPropertyDomain(modsci:appliesLawsFrom modsci:ModernScience)
ObjectPropertyRange(modsci:appliesLawsFrom modsci:ModernScience)

# Object Property: modsci:appliesLawsFromMathematics (modsci:appliesLawsFromMathematics)

SubObjectPropertyOf(modsci:appliesLawsFromMathematics modsci:appliesLawsFrom)

# Object Property: modsci:appliesLawsFromPhysics (modsci:appliesLawsFromPhysics)

SubObjectPropertyOf(modsci:appliesLawsFromPhysics modsci:appliesLawsFrom)

# Object Property: modsci:appliesLawsFromStatistics (modsci:appliesLawsFromStatistics)

SubObjectPropertyOf(modsci:appliesLawsFromStatistics modsci:appliesLawsFrom)

# Object Property: modsci:appliesLawsFromThermodynamics (modsci:appliesLawsFromThermodynamics)

SubObjectPropertyOf(modsci:appliesLawsFromThermodynamics modsci:appliesLawsFromPhysics)

# Object Property: modsci:discoveredByAppliedSciences (modsci:discoveredByAppliedSciences)

SubObjectPropertyOf(modsci:discoveredByAppliedSciences modsci:discoveredByScience)

# Object Property: modsci:discoveredByBehaviouralSciences (modsci:discoveredByBehaviouralSciences)

SubObjectPropertyOf(modsci:discoveredByBehaviouralSciences modsci:discoveredByScience)

# Object Property: modsci:discoveredByFormalScience (modsci:discoveredByFormalScience)

SubObjectPropertyOf(modsci:discoveredByFormalScience modsci:discoveredByScience)

# Object Property: modsci:discoveredByHealthSciences (modsci:discoveredByHealthSciences)

SubObjectPropertyOf(modsci:discoveredByHealthSciences modsci:discoveredByScience)

# Object Property: modsci:discoveredByInterdisciplinaryStudies (modsci:discoveredByInterdisciplinaryStudies)

SubObjectPropertyOf(modsci:discoveredByInterdisciplinaryStudies modsci:discoveredByScience)

# Object Property: modsci:discoveredByMachine (modsci:discoveredByMachine)

SubObjectPropertyOf(modsci:discoveredByMachine owl:topObjectProperty)

# Object Property: modsci:discoveredByNaturalScience (modsci:discoveredByNaturalScience)

SubObjectPropertyOf(modsci:discoveredByNaturalScience modsci:discoveredByScience)

# Object Property: modsci:discoveredByScience (modsci:discoveredByScience)

FunctionalObjectProperty(modsci:discoveredByScience)
ObjectPropertyDomain(modsci:discoveredByScience ObjectUnionOf(sweet:Phenomenon modsci:ScientificDiscovery))
ObjectPropertyRange(modsci:discoveredByScience modsci:ModernScience)

# Object Property: modsci:discoveredByScientist (modsci:discoveredByScientist)

FunctionalObjectProperty(modsci:discoveredByScientist)
ObjectPropertyDomain(modsci:discoveredByScientist ObjectUnionOf(sweet:Phenomenon modsci:ScientificDiscovery))
ObjectPropertyDomain(modsci:discoveredByScientist ObjectMinCardinality(1 modsci:discoveredByScientist modsci:Scientist))
ObjectPropertyRange(modsci:discoveredByScientist modsci:Scientist)
ObjectPropertyRange(modsci:discoveredByScientist ObjectAllValuesFrom(modsci:discoveredByScientist modsci:Scientist))

# Object Property: modsci:discoveredBySocialSciences (modsci:discoveredBySocialSciences)

SubObjectPropertyOf(modsci:discoveredBySocialSciences modsci:discoveredByScience)

# Object Property: modsci:followsMethod (modsci:followsMethod)

ObjectPropertyDomain(modsci:followsMethod modsci:Scientist)
ObjectPropertyRange(modsci:followsMethod modsci:ScientificMethod)

# Object Property: modsci:hasApplication (modsci:hasApplication)

InverseObjectProperties(modsci:hasApplication modsci:isApplicationOfScience)
ObjectPropertyDomain(modsci:hasApplication modsci:ModernScience)
ObjectPropertyRange(modsci:hasApplication modsci:ApplicationOfScience)

# Object Property: modsci:hasCloseRelationshipTo (modsci:hasCloseRelationshipTo)

SymmetricObjectProperty(modsci:hasCloseRelationshipTo)
ReflexiveObjectProperty(modsci:hasCloseRelationshipTo)
ObjectPropertyDomain(modsci:hasCloseRelationshipTo modsci:ModernScience)
ObjectPropertyRange(modsci:hasCloseRelationshipTo modsci:ModernScience)

# Object Property: modsci:hasCollaborationWith (modsci:hasCollaborationWith)

SymmetricObjectProperty(modsci:hasCollaborationWith)
ReflexiveObjectProperty(modsci:hasCollaborationWith)
ObjectPropertyDomain(modsci:hasCollaborationWith modsci:ModernScience)
ObjectPropertyRange(modsci:hasCollaborationWith modsci:ModernScience)

# Object Property: modsci:hasManufacturer (modsci:hasManufacturer)

InverseObjectProperties(modsci:hasManufacturer modsci:isManufacturerOf)
ObjectPropertyDomain(modsci:hasManufacturer modsci:ScientificInstrument)
ObjectPropertyRange(modsci:hasManufacturer modsci:ScientificInstrumentManufacturer)

# Object Property: modsci:hasMethodsInspiredFrom (modsci:hasMethodsInspiredFrom)

ReflexiveObjectProperty(modsci:hasMethodsInspiredFrom)
ObjectPropertyDomain(modsci:hasMethodsInspiredFrom modsci:ModernScience)
ObjectPropertyRange(modsci:hasMethodsInspiredFrom modsci:ModernScience)

# Object Property: modsci:hasScientificInstrumentManufacturer (modsci:hasScientificInstrumentManufacturer)

SubObjectPropertyOf(modsci:hasScientificInstrumentManufacturer modsci:hasManufacturer)

# Object Property: modsci:inspiredFrom (modsci:inspiredFrom)

FunctionalObjectProperty(modsci:inspiredFrom)
ObjectPropertyDomain(modsci:inspiredFrom modsci:ScientificMethod)
ObjectPropertyRange(modsci:inspiredFrom ObjectUnionOf(sweet:Phenomenon modsci:ScientificDiscovery))

# Object Property: modsci:inspiredFromPhenomenon (modsci:inspiredFromPhenomenon)

SubObjectPropertyOf(modsci:inspiredFromPhenomenon modsci:inspiredFrom)

# Object Property: modsci:inspiredFromScientificDiscovery (modsci:inspiredFromScientificDiscovery)

SubObjectPropertyOf(modsci:inspiredFromScientificDiscovery modsci:inspiredFrom)

# Object Property: modsci:instrumentInventedBy (modsci:instrumentInventedBy)

ObjectPropertyDomain(modsci:instrumentInventedBy modsci:ScientificInstrument)
ObjectPropertyRange(modsci:instrumentInventedBy modsci:Scientist)

# Object Property: modsci:instrumentUsedInScience (instrument used in Science)

AnnotationAssertion(rdfs:label modsci:instrumentUsedInScience "instrument used in Science")
ObjectPropertyDomain(modsci:instrumentUsedInScience modsci:ScientificInstrument)
ObjectPropertyRange(modsci:instrumentUsedInScience modsci:ModernScience)

# Object Property: modsci:interestedInPhenomenon (modsci:interestedInPhenomenon)

ObjectPropertyDomain(modsci:interestedInPhenomenon modsci:Scientist)
ObjectPropertyRange(modsci:interestedInPhenomenon sweet:Phenomenon)

# Object Property: modsci:isApplicationOfAppliedScience (modsci:isApplicationOfAppliedScience)

SubObjectPropertyOf(modsci:isApplicationOfAppliedScience modsci:isApplicationOfScience)

# Object Property: modsci:isApplicationOfBehaviouralSciences (modsci:isApplicationOfBehaviouralSciences)

SubObjectPropertyOf(modsci:isApplicationOfBehaviouralSciences modsci:isApplicationOfScience)

# Object Property: modsci:isApplicationOfFormalScience (modsci:isApplicationOfFormalScience)

SubObjectPropertyOf(modsci:isApplicationOfFormalScience modsci:isApplicationOfScience)

# Object Property: modsci:isApplicationOfHealthSciences (modsci:isApplicationOfHealthSciences)

SubObjectPropertyOf(modsci:isApplicationOfHealthSciences modsci:isApplicationOfScience)

# Object Property: modsci:isApplicationOfInterdisciplinaryStudies (modsci:isApplicationOfInterdisciplinaryStudies)

SubObjectPropertyOf(modsci:isApplicationOfInterdisciplinaryStudies modsci:isApplicationOfScience)

# Object Property: modsci:isApplicationOfNaturalScience (modsci:isApplicationOfNaturalScience)

SubObjectPropertyOf(modsci:isApplicationOfNaturalScience modsci:isApplicationOfScience)

# Object Property: modsci:isApplicationOfScience (modsci:isApplicationOfScience)

ObjectPropertyDomain(modsci:isApplicationOfScience modsci:ApplicationOfScience)
ObjectPropertyRange(modsci:isApplicationOfScience modsci:ModernScience)

# Object Property: modsci:isApplicationOfSocialSciences (modsci:isApplicationOfSocialSciences)

SubObjectPropertyOf(modsci:isApplicationOfSocialSciences modsci:isApplicationOfScience)

# Object Property: modsci:isDiscoveredBy (modsci:isDiscoveredBy)

IrreflexiveObjectProperty(modsci:isDiscoveredBy)
ObjectPropertyDomain(modsci:isDiscoveredBy ObjectUnionOf(sweet:Phenomenon modsci:ScientificDiscovery))
ObjectPropertyRange(modsci:isDiscoveredBy ObjectUnionOf(modsci:ScientificOrganization modsci:Scientist))

# Object Property: modsci:isDiscoveredByOrganization (modsci:isDiscoveredByOrganization)

SubObjectPropertyOf(modsci:isDiscoveredByOrganization modsci:isDiscoveredBy)

# Object Property: modsci:isDiscoveredByScientist (modsci:isDiscoveredByScientist)

SubObjectPropertyOf(modsci:isDiscoveredByScientist modsci:isDiscoveredBy)

# Object Property: modsci:isStudentOf (modsci:isStudentOf)

ObjectPropertyDomain(modsci:isStudentOf modsci:Scientist)
ObjectPropertyRange(modsci:isStudentOf modsci:Scientist)

# Object Property: modsci:requiresKnowledgeFrom (modsci:requiresKnowledgeFrom)

ReflexiveObjectProperty(modsci:requiresKnowledgeFrom)
ObjectPropertyDomain(modsci:requiresKnowledgeFrom modsci:ModernScience)
ObjectPropertyRange(modsci:requiresKnowledgeFrom modsci:ModernScience)

# Object Property: modsci:scientistBelongsTo (modsci:scientistBelongsTo)

ObjectPropertyDomain(modsci:scientistBelongsTo modsci:Scientist)
ObjectPropertyRange(modsci:scientistBelongsTo modsci:ModernScience)

# Object Property: modsci:suppliesSubstancesTo (modsci:suppliesSubstancesTo)

InverseObjectProperties(modsci:suppliesSubstancesTo modsci:takeSunstancesFrom)
ReflexiveObjectProperty(modsci:suppliesSubstancesTo)
ObjectPropertyDomain(modsci:suppliesSubstancesTo modsci:ModernScience)
ObjectPropertyRange(modsci:suppliesSubstancesTo ObjectUnionOf(modsci:Industry modsci:ModernScience))

# Object Property: modsci:takeSunstancesFrom (modsci:takeSunstancesFrom)

ReflexiveObjectProperty(modsci:takeSunstancesFrom)
ObjectPropertyDomain(modsci:takeSunstancesFrom modsci:ModernScience)
ObjectPropertyRange(modsci:takeSunstancesFrom modsci:ModernScience)

# Object Property: modsci:undertakesResearch (modsci:undertakesResearch)

ObjectPropertyDomain(modsci:undertakesResearch modsci:Scientist)
ObjectPropertyRange(modsci:undertakesResearch modsci:ModernScience)

# Object Property: modsci:usesMethodsFrom (modsci:usesMethodsFrom)

ReflexiveObjectProperty(modsci:usesMethodsFrom)
ObjectPropertyDomain(modsci:usesMethodsFrom modsci:ModernScience)
ObjectPropertyRange(modsci:usesMethodsFrom modsci:ModernScience)

# Object Property: modsci:usesTechniquesFrom (modsci:usesTechniquesFrom)

ReflexiveObjectProperty(modsci:usesTechniquesFrom)
ObjectPropertyDomain(modsci:usesTechniquesFrom modsci:ModernScience)
ObjectPropertyRange(modsci:usesTechniquesFrom modsci:ModernScience)


############################
#   Data Properties
############################

# Data Property: modsci:InstrumentFunctionDesription (modsci:InstrumentFunctionDesription)

DataPropertyDomain(modsci:InstrumentFunctionDesription modsci:ScientificInstrument)
DataPropertyRange(modsci:InstrumentFunctionDesription xsd:string)



############################
#   Classes
############################

# Class: sweet:Phenomenon (Phenomenon)

AnnotationAssertion(rdfs:comment sweet:Phenomenon "A phenomenon, in a scientific context, is something that is observed to occur or to exist."@en)
AnnotationAssertion(rdfs:label sweet:Phenomenon "Phenomenon"@en)

# Class: modsci:AcidbaseChemistry (Acid–base Chemistry)

AnnotationAssertion(rdfs:comment modsci:AcidbaseChemistry "For chemicals that can behave as acids or bases")
AnnotationAssertion(rdfs:label modsci:AcidbaseChemistry "Acid–base Chemistry")
SubClassOf(modsci:AcidbaseChemistry modsci:Chemistry)

# Class: modsci:Acoustics (Acoustics)

AnnotationAssertion(rdfs:comment modsci:Acoustics "Acoustics is a branch of continuum mechanics and is the study of sound, mechanical waves in gases, liquids, and solids.")
AnnotationAssertion(rdfs:label modsci:Acoustics "Acoustics")
SubClassOf(modsci:Acoustics modsci:ClassicalPhysics)

# Class: modsci:Agriculture (Agriculture)

AnnotationAssertion(rdfs:comment modsci:Agriculture "Agriculture, also known as farming, is the process of producing food, feed, fiber and other desired products by cultivation of certain plants and the raising of domesticated animals.")
AnnotationAssertion(rdfs:label modsci:Agriculture "Agriculture")
SubClassOf(modsci:Agriculture modsci:AppliedSciences)

# Class: modsci:Agronomy (modsci:Agronomy)

SubClassOf(modsci:Agronomy modsci:Agriculture)

# Class: modsci:Algebra (modsci:Algebra)

SubClassOf(modsci:Algebra modsci:PureMathematics)

# Class: modsci:Algorithms (Algorithms)

AnnotationAssertion(rdfs:label modsci:Algorithms "Algorithms")
SubClassOf(modsci:Algorithms modsci:ScientificMethod)

# Class: modsci:AnalyticalChemistry (Analytical Chemistry)

AnnotationAssertion(rdfs:comment modsci:AnalyticalChemistry "Analytical chemistry is the analysis of material samples to gain an understanding of their chemical composition and structure.")
AnnotationAssertion(rdfs:label modsci:AnalyticalChemistry "Analytical Chemistry")
SubClassOf(modsci:AnalyticalChemistry modsci:Chemistry)

# Class: modsci:AnalyticalSpectrometry (modsci:AnalyticalSpectrometry)

SubClassOf(modsci:AnalyticalSpectrometry modsci:AnalyticalChemistry)

# Class: modsci:Anatomy (Anatomy)

AnnotationAssertion(rdfs:comment modsci:Anatomy "Anatomy is the study of the structure and organization of living things.")
AnnotationAssertion(rdfs:label modsci:Anatomy "Anatomy")
SubClassOf(modsci:Anatomy modsci:Biology)

# Class: modsci:AnimalProduction (modsci:AnimalProduction)

SubClassOf(modsci:AnimalProduction modsci:Agriculture)

# Class: modsci:Anthropology (Anthropology)

AnnotationAssertion(rdfs:comment modsci:Anthropology "Anthropology is the scientific study of humans, human behavior and societies in the past and present.")
AnnotationAssertion(rdfs:label modsci:Anthropology "Anthropology")
SubClassOf(modsci:Anthropology modsci:SocialSciences)

# Class: modsci:ApplicationOfScience (Application of science)

AnnotationAssertion(rdfs:comment modsci:ApplicationOfScience "An application of science is any use of scientific knowledge for a specific purpose, whether to do more science; to design a product, process, or medical treatment; to develop a new technology; or to predict the impacts of human actions.")
AnnotationAssertion(rdfs:label modsci:ApplicationOfScience "Application of science")

# Class: modsci:AppliedMathematics (Applied Mathematics)

AnnotationAssertion(rdfs:comment modsci:AppliedMathematics "Applied mathematics is a branch of mathematics that concerns itself with the application of mathematical knowledge to other domains.")
AnnotationAssertion(rdfs:label modsci:AppliedMathematics "Applied Mathematics")
SubClassOf(modsci:AppliedMathematics modsci:Mathematics)

# Class: modsci:AppliedMechanics (modsci:AppliedMechanics)

SubClassOf(modsci:AppliedMechanics modsci:AppliedMathematics)

# Class: modsci:AppliedPhysics (Applied and Interdisciplinary Physics)

AnnotationAssertion(rdfs:comment modsci:AppliedPhysics "Applied physics is intended for a particular technological or practical use.")
AnnotationAssertion(rdfs:label modsci:AppliedPhysics "Applied and Interdisciplinary Physics")
SubClassOf(modsci:AppliedPhysics modsci:InterdisciplinaryStudies)
SubClassOf(modsci:AppliedPhysics modsci:Physics)

# Class: modsci:AppliedSciences (Applied Sciences)

AnnotationAssertion(rdfs:comment modsci:AppliedSciences "Applied science is the use or the study of the use of scientific knowledge to develop technology.")
AnnotationAssertion(rdfs:label modsci:AppliedSciences "Applied Sciences")
SubClassOf(modsci:AppliedSciences modsci:ModernScience)

# Class: modsci:ApproximationTheory (modsci:ApproximationTheory)

SubClassOf(modsci:ApproximationTheory modsci:AppliedMathematics)

# Class: modsci:Archaeology (Archaeology)

AnnotationAssertion(rdfs:comment modsci:Archaeology "Archaeology, or archeology, is the study of human activity through the recovery and analysis of material culture.")
AnnotationAssertion(rdfs:label modsci:Archaeology "Archaeology")
SubClassOf(modsci:Archaeology modsci:SocialSciences)

# Class: modsci:Architecture (Architecture)

AnnotationAssertion(rdfs:comment modsci:Architecture "Architecture is the art and science of designing buildings.")
AnnotationAssertion(rdfs:label modsci:Architecture "Architecture")
SubClassOf(modsci:Architecture modsci:AppliedSciences)

# Class: modsci:ArtificialIntelligence (Artificial Intelligence)

AnnotationAssertion(rdfs:comment modsci:ArtificialIntelligence "In computer science, artificial intelligence (AI), sometimes called machine intelligence, is intelligence demonstrated by machines, in contrast to the natural intelligence displayed by humans. Colloquially, the term \"artificial intelligence\" is often used to describe machines (or computers) that mimic \"cognitive\" functions that humans associate with the human mind, such as \"learning\" and \"problem solving\".")
AnnotationAssertion(rdfs:label modsci:ArtificialIntelligence "Artificial Intelligence")
SubClassOf(modsci:ArtificialIntelligence modsci:ComputerScience)

# Class: modsci:Astrobiology (Astrobiology)

AnnotationAssertion(rdfs:comment modsci:Astrobiology "Astrobiology, formerly known as exobiology, is an interdisciplinary scientific field concerned with the origins, early evolution, distribution, and future of life in the universe.")
AnnotationAssertion(rdfs:label modsci:Astrobiology "Astrobiology")
SubClassOf(modsci:Astrobiology modsci:Biology)

# Class: modsci:Astrochemistry (Astrochemistry)

AnnotationAssertion(rdfs:comment modsci:Astrochemistry "Astrochemistry is the study of the abundance and reactions of molecules in the Universe, and their interaction with radiation.")
AnnotationAssertion(rdfs:label modsci:Astrochemistry "Astrochemistry")
SubClassOf(modsci:Astrochemistry modsci:Chemistry)

# Class: modsci:Astrometry (Astrometry)

AnnotationAssertion(rdfs:comment modsci:Astrometry "Astrometry is the study of the positions, distances between, and motions of astronomical objects.")
AnnotationAssertion(rdfs:label modsci:Astrometry "Astrometry")
SubClassOf(modsci:Astrometry modsci:Astronomy)

# Class: modsci:AstronomicalPhenomena (Astronomical Phenomena)

AnnotationAssertion(rdfs:label modsci:AstronomicalPhenomena "Astronomical Phenomena")
SubClassOf(modsci:AstronomicalPhenomena modsci:NaturalPhenomenon)

# Class: modsci:Astronomy (Astronomy)

AnnotationAssertion(rdfs:comment modsci:Astronomy "is a science involving the observation and explanation of events occurring outside Earth and its atmosphere.")
AnnotationAssertion(rdfs:label modsci:Astronomy "Astronomy")
SubClassOf(modsci:Astronomy modsci:NaturalScience)

# Class: modsci:AtmosphericPhenomena (Atmospheric Optical Phenomena)

AnnotationAssertion(rdfs:label modsci:AtmosphericPhenomena "Atmospheric Optical Phenomena")
SubClassOf(modsci:AtmosphericPhenomena modsci:NaturalPhenomenon)

# Class: modsci:AtmosphericSciences (Atmospheric Sciences)

AnnotationAssertion(rdfs:comment modsci:AtmosphericSciences "Atmospheric science is an umbrella term for the study of the atmosphere and its processes.")
AnnotationAssertion(rdfs:label modsci:AtmosphericSciences "Atmospheric Sciences")
SubClassOf(modsci:AtmosphericSciences modsci:EarthScience)

# Class: modsci:AtomicPhysics (Atomic, Molecular, and Optical Physics)

AnnotationAssertion(rdfs:comment modsci:AtomicPhysics "Atomic, molecular, and optical physics (AMO) is the study of matter-matter and light-matter interactions; at the scale of one or a few atoms and energy scales around several electron volts.")
AnnotationAssertion(rdfs:label modsci:AtomicPhysics "Atomic, Molecular, and Optical Physics")
EquivalentClasses(modsci:AtomicPhysics modsci:MolecularPhysics)
SubClassOf(modsci:AtomicPhysics modsci:Physics)

# Class: modsci:AutomataTheory (Automata Theory)

AnnotationAssertion(rdfs:comment modsci:AutomataTheory "Automata theory is the study of abstract machines and automata, as well as the computational problems that can be solved using them.")
AnnotationAssertion(rdfs:label modsci:AutomataTheory "Automata Theory")
SubClassOf(modsci:AutomataTheory modsci:TheoryOfComputation)

# Class: modsci:AutomatedReasoning (Automated Reasoning)

AnnotationAssertion(rdfs:comment modsci:AutomatedReasoning "Automated reasoning is an area of computer science, cognitive science, and mathematical logic dedicated to understanding different aspects of reasoning.")
AnnotationAssertion(rdfs:label modsci:AutomatedReasoning "Automated Reasoning")
SubClassOf(modsci:AutomatedReasoning modsci:ArtificialIntelligence)

# Class: modsci:BasinAnalysis (modsci:BasinAnalysis)

SubClassOf(modsci:BasinAnalysis modsci:Geology)

# Class: modsci:BehaviouralSciences (Behavioural Sciences)

AnnotationAssertion(rdfs:comment modsci:BehaviouralSciences "Behavioural sciences explore the cognitive processes within organisms and the behavioural interactions between organisms in the natural world.")
AnnotationAssertion(rdfs:label modsci:BehaviouralSciences "Behavioural Sciences")
SubClassOf(modsci:BehaviouralSciences modsci:ModernScience)

# Class: modsci:Biochemistry (Biochemistry)

AnnotationAssertion(rdfs:comment modsci:Biochemistry "Biochemistry is the chemistry of life.")
AnnotationAssertion(rdfs:label modsci:Biochemistry "Biochemistry")
SubClassOf(modsci:Biochemistry modsci:Biology)
SubClassOf(modsci:Biochemistry modsci:Chemistry)

# Class: modsci:Bioengineering (Biological Engineering)

AnnotationAssertion(rdfs:comment modsci:Bioengineering "Biological engineering, or bioengineering/bio-engineering, is the application of principles of biology and the tools of engineering to create usable, tangible, economically viable products.")
AnnotationAssertion(rdfs:label modsci:Bioengineering "Biological Engineering")
SubClassOf(modsci:Bioengineering modsci:Biology)
SubClassOf(modsci:Bioengineering modsci:Engineering)

# Class: modsci:Bioethics (Bioethics)

AnnotationAssertion(rdfs:comment modsci:Bioethics "Bioethics is the study of the ethical issues emerging from advances in biology and medicine.")
AnnotationAssertion(rdfs:label modsci:Bioethics "Bioethics")
SubClassOf(modsci:Bioethics modsci:Biology)

# Class: modsci:Biogeography (Biogeography)

AnnotationAssertion(rdfs:comment modsci:Biogeography "Biogeography is the study of the distribution of species and ecosystems in geographic space and through geological time.")
AnnotationAssertion(rdfs:label modsci:Biogeography "Biogeography")
SubClassOf(modsci:Biogeography modsci:Biology)

# Class: modsci:Bioinformatics (Bioinformatics)

AnnotationAssertion(rdfs:comment modsci:Bioinformatics "Bioinformatics and Computational biology are interdisciplinary fields of research, development and application of algorithms, computational and statistical methods for management and analysis of biological data, and for solving basic biological problems.")
AnnotationAssertion(rdfs:label modsci:Bioinformatics "Bioinformatics")
SubClassOf(modsci:Bioinformatics modsci:Biology)
SubClassOf(modsci:Bioinformatics modsci:InterdisciplinaryStudies)

# Class: modsci:BioinformaticsSoftware (modsci:BioinformaticsSoftware)

SubClassOf(modsci:BioinformaticsSoftware modsci:ComputerSoftware)

# Class: modsci:BioinorganicChemistry (modsci:BioinorganicChemistry)

SubClassOf(modsci:BioinorganicChemistry modsci:InorganicChemistry)

# Class: modsci:BiologicalMathematics (modsci:BiologicalMathematics)

SubClassOf(modsci:BiologicalMathematics modsci:AppliedMathematics)

# Class: modsci:BiologicalOceanography (modsci:BiologicalOceanography)

SubClassOf(modsci:BiologicalOceanography modsci:Oceanography)

# Class: modsci:BiologicalPhenomena (Biological Phenomena)

AnnotationAssertion(rdfs:label modsci:BiologicalPhenomena "Biological Phenomena")
SubClassOf(modsci:BiologicalPhenomena modsci:NaturalPhenomenon)

# Class: modsci:Biology (Biology)

AnnotationAssertion(rdfs:comment modsci:Biology "Biology is the science of life. It is concerned with the characteristics and behaviors of organisms")
AnnotationAssertion(rdfs:label modsci:Biology "Biology")
SubClassOf(modsci:Biology modsci:NaturalScience)

# Class: modsci:BiomedicalEngineering (Biomedical Engineering)

AnnotationAssertion(rdfs:comment modsci:BiomedicalEngineering "Biomedical engineering (BME) or medical engineering is the application of engineering principles and design concepts to medicine and biology for healthcare purposes (e.g. diagnostic or therapeutic).")
AnnotationAssertion(rdfs:label modsci:BiomedicalEngineering "Biomedical Engineering")
SubClassOf(modsci:BiomedicalEngineering modsci:InterdisciplinaryStudies)

# Class: modsci:Biophysics (Biophysics)

AnnotationAssertion(rdfs:comment modsci:Biophysics "Biophysics is an interdisciplinary science that applies approaches and methods traditionally used in physics to study biological phenomena.")
AnnotationAssertion(rdfs:label modsci:Biophysics "Biophysics")
SubClassOf(modsci:Biophysics modsci:Biology)

# Class: modsci:Biopsychology (Biopsychology)

AnnotationAssertion(rdfs:comment modsci:Biopsychology "Biological psychology,is the application of the principles of biology to the study of physiological and developmental mechanisms of behavior in humans and other animals.")
AnnotationAssertion(rdfs:label modsci:Biopsychology "Biopsychology")
SubClassOf(modsci:Biopsychology modsci:Biology)

# Class: modsci:Biostatistics (Biostatistics)

AnnotationAssertion(rdfs:comment modsci:Biostatistics "Biostatistics are the development and application of statistical methods to a wide range of topics in biology.")
AnnotationAssertion(rdfs:label modsci:Biostatistics "Biostatistics")
SubClassOf(modsci:Biostatistics modsci:Biology)

# Class: modsci:Biotechnology (Biotechnology)

AnnotationAssertion(rdfs:comment modsci:Biotechnology "Biotechnology is a technology based on biology, especially when used in agriculture, food science, medicine, and genetic engineering.")
AnnotationAssertion(rdfs:label modsci:Biotechnology "Biotechnology")
SubClassOf(modsci:Biotechnology modsci:Biology)

# Class: modsci:Botany (Botany)

AnnotationAssertion(rdfs:comment modsci:Botany "Botany also called plant science(s), plant biology or phytology, is the science of plant life and a branch of biology.")
AnnotationAssertion(rdfs:label modsci:Botany "Botany")
SubClassOf(modsci:Botany modsci:Biology)

# Class: modsci:CalculusOfVariations (modsci:CalculusOfVariations)

SubClassOf(modsci:CalculusOfVariations modsci:AppliedMathematics)

# Class: modsci:Catalysis (modsci:Catalysis)

SubClassOf(modsci:Catalysis modsci:PhysicalChemistry)

# Class: modsci:CellBiology (Cell Biology)

AnnotationAssertion(rdfs:comment modsci:CellBiology "Cell biology is a branch of biology that studies the structure and function of the cell, which is the basic unit of life.")
AnnotationAssertion(rdfs:label modsci:CellBiology "Cell Biology")
SubClassOf(modsci:CellBiology modsci:Biology)

# Class: modsci:ChemicalCharacterisationOfMaterials (modsci:ChemicalCharacterisationOfMaterials)

SubClassOf(modsci:ChemicalCharacterisationOfMaterials modsci:MaterialsChemistry)

# Class: modsci:ChemicalEngineering (Chemical Engineering)

AnnotationAssertion(rdfs:comment modsci:ChemicalEngineering "Chemical engineering is the application of science, in particular chemistry, fluid physics, and biology, along with mathematics and economics to the human endeavor of converting raw materials or chemicals into more useful or valuable forms.")
AnnotationAssertion(rdfs:label modsci:ChemicalEngineering "Chemical Engineering")
SubClassOf(modsci:ChemicalEngineering modsci:Chemistry)

# Class: modsci:ChemicalOceanography (modsci:ChemicalOceanography)

SubClassOf(modsci:ChemicalOceanography modsci:Oceanography)

# Class: modsci:ChemicalPhenomena (Chemical Phenomena)

AnnotationAssertion(rdfs:label modsci:ChemicalPhenomena "Chemical Phenomena")
SubClassOf(modsci:ChemicalPhenomena modsci:NaturalPhenomenon)

# Class: modsci:ChemicalThermodynamics (modsci:ChemicalThermodynamics)

SubClassOf(modsci:ChemicalThermodynamics modsci:PhysicalChemistry)

# Class: modsci:Chemistry (Chemistry)

AnnotationAssertion(rdfs:comment modsci:Chemistry "Chemistry is defined as the science of matter, different from physics, in terms of matter's chemical structure, reactivity, properties and reactions or transformations.")
AnnotationAssertion(rdfs:label modsci:Chemistry "Chemistry")
SubClassOf(modsci:Chemistry modsci:NaturalScience)

# Class: modsci:ClassicalPhysics (modsci:ClassicalPhysics)

SubClassOf(modsci:ClassicalPhysics modsci:Physics)

# Class: modsci:ClassificationAlgorithms (modsci:ClassificationAlgorithms)

SubClassOf(modsci:ClassificationAlgorithms modsci:Algorithms)

# Class: modsci:CoalGeology (modsci:CoalGeology)

SubClassOf(modsci:CoalGeology modsci:Geology)

# Class: modsci:CodingAndInformationTheory (modsci:CodingAndInformationTheory)

SubClassOf(modsci:CodingAndInformationTheory modsci:DataFormat)

# Class: modsci:CognitiveScience (Cognitive Science)

AnnotationAssertion(rdfs:comment modsci:CognitiveScience "Cognitive science is the interdisciplinary, scientific study of the mind and its processes.")
AnnotationAssertion(rdfs:label modsci:CognitiveScience "Cognitive Science")
SubClassOf(modsci:CognitiveScience modsci:InterdisciplinaryStudies)

# Class: modsci:Colloid (modsci:Colloid)

SubClassOf(modsci:Colloid modsci:PhysicalChemistry)

# Class: modsci:ColloidalChemistry (Colloidal Chemistry)

AnnotationAssertion(rdfs:comment modsci:ColloidalChemistry "Interface and colloid science is an interdisciplinary intersection of branches of chemistry, physics, nanoscience and other fields dealing with colloids, heterogeneous systems consisting of a mechanical mixture of particles between 1 nm and 1000 nm dispersed in a continuous medium.")
AnnotationAssertion(rdfs:label modsci:ColloidalChemistry "Colloidal Chemistry")
SubClassOf(modsci:ColloidalChemistry modsci:Chemistry)

# Class: modsci:CommunicationAndSecurity (Communication and Security)

AnnotationAssertion(rdfs:comment modsci:CommunicationAndSecurity "Communications security is the discipline of preventing unauthorized interceptors from accessing telecommunications in an intelligible form, while still delivering content to the intended recipients.")
AnnotationAssertion(rdfs:label modsci:CommunicationAndSecurity "Communication and Security")
SubClassOf(modsci:CommunicationAndSecurity modsci:ComputerSoftware)

# Class: modsci:CommunicationStudies (Communication)

AnnotationAssertion(rdfs:comment modsci:CommunicationStudies "Communication is the act of conveying meanings from one entity or group to another through the use of mutually understood signs, symbols, and semiotic rules.")
AnnotationAssertion(rdfs:label modsci:CommunicationStudies "Communication")
SubClassOf(modsci:CommunicationStudies modsci:SocialSciences)

# Class: modsci:CompilerTheory (Compiler Theory)

AnnotationAssertion(rdfs:comment modsci:CompilerTheory "A compiler implements a formal transformation from a high-level source program to a low-level target program.")
AnnotationAssertion(rdfs:label modsci:CompilerTheory "Compiler Theory")
SubClassOf(modsci:CompilerTheory modsci:ProgrammingLanguages)

# Class: modsci:ComputabilityTheory (Computability Theory)

AnnotationAssertion(rdfs:comment modsci:ComputabilityTheory "Computability theory, also known as recursion theory, is a branch of mathematical logic, of computer science, and of the theory of computation that originated in the 1930s with the study of computable functions and Turing degrees.")
AnnotationAssertion(rdfs:label modsci:ComputabilityTheory "Computability Theory")
SubClassOf(modsci:ComputabilityTheory modsci:TheoryOfComputation)

# Class: modsci:ComputationalComplexityTheory (Computational Complexity Theory)

AnnotationAssertion(rdfs:comment modsci:ComputationalComplexityTheory "Computational complexity theory focuses on classifying computational problems according to their inherent difficulty, and relating these classes to each other. A computational problem is a task solved by a computer.")
AnnotationAssertion(rdfs:label modsci:ComputationalComplexityTheory "Computational Complexity Theory")
SubClassOf(modsci:ComputationalComplexityTheory modsci:TheoryOfComputation)

# Class: modsci:ComputationalLinguistics (Computational Linguistics)

AnnotationAssertion(rdfs:comment modsci:ComputationalLinguistics "Computational linguistics is an interdisciplinary field concerned with the statistical or rule-based modeling of natural language from a computational perspective, as well as the study of appropriate computational approaches to linguistic questions.")
AnnotationAssertion(rdfs:label modsci:ComputationalLinguistics "Computational Linguistics")
SubClassOf(modsci:ComputationalLinguistics modsci:InterdisciplinaryStudies)

# Class: modsci:ComputationalMathematics (modsci:ComputationalMathematics)

SubClassOf(modsci:ComputationalMathematics modsci:Mathematics)

# Class: modsci:ComputationalPhysics (Computational Physics)

AnnotationAssertion(rdfs:comment modsci:ComputationalPhysics "Computational physics is the study and implementation of numerical algorithms in order to solve problems in physics for which a quantitative theory already exists.")
AnnotationAssertion(rdfs:label modsci:ComputationalPhysics "Computational Physics")
SubClassOf(modsci:ComputationalPhysics modsci:Physics)

# Class: modsci:Computer-HumanInteraction (modsci:Computer-HumanInteraction)

SubClassOf(modsci:Computer-HumanInteraction modsci:InformationSystems)

# Class: modsci:ComputerApplications (modsci:ComputerApplications)

SubClassOf(modsci:ComputerApplications modsci:ComputerScience)

# Class: modsci:ComputerConcurrency (Computer Concurrency)

AnnotationAssertion(rdfs:comment modsci:ComputerConcurrency "In computer science, concurrency is the ability of different parts or units of a program, algorithm, or problem to be executed out-of-order or in partial order, without affecting the final outcome. This allows for parallel execution of the concurrent units, which can significantly improve overall speed of the execution in multi-processor and multi-core systems.")
AnnotationAssertion(rdfs:label modsci:ComputerConcurrency "Computer Concurrency")
SubClassOf(modsci:ComputerConcurrency modsci:DistributedSystems)

# Class: modsci:ComputerGraphics (Graphics)

AnnotationAssertion(rdfs:comment modsci:ComputerGraphics "Computer graphics are pictures and films created using computers. Usually, the term refers to computer-generated image data created with the help of specialized graphical hardware and software.")
AnnotationAssertion(rdfs:comment modsci:ComputerGraphics "Computer graphics is the study of digital visual contents and involves the synthesis and manipulation of image data.")
AnnotationAssertion(rdfs:label modsci:ComputerGraphics "Computer Graphics")
AnnotationAssertion(rdfs:label modsci:ComputerGraphics "Graphics")
SubClassOf(modsci:ComputerGraphics modsci:ComputerGraphics)
SubClassOf(modsci:ComputerGraphics modsci:ImageProcessing)

# Class: modsci:ComputerScience (Computer Science)

AnnotationAssertion(rdfs:comment modsci:ComputerScience "Computer science is the study of processes that interact with data and that can be represented as data in the form of programs.")
AnnotationAssertion(rdfs:label modsci:ComputerScience "Computer Science")
SubClassOf(modsci:ComputerScience modsci:AppliedSciences)

# Class: modsci:ComputerSecurity (Computer Security)

AnnotationAssertion(rdfs:comment modsci:ComputerSecurity "Computer security, cybersecurity or information technology security (IT security) is the protection of computer systems from the theft of or damage to their hardware, software, or electronic data, as well as from the disruption or misdirection of the services they provide.")
AnnotationAssertion(rdfs:label modsci:ComputerSecurity "Computer Security")
SubClassOf(modsci:ComputerSecurity modsci:CommunicationAndSecurity)

# Class: modsci:ComputerSoftware (modsci:ComputerSoftware)

SubClassOf(modsci:ComputerSoftware modsci:ComputerScience)

# Class: modsci:ComputerSystemArchitecture (Computer Architecture)

AnnotationAssertion(rdfs:comment modsci:ComputerSystemArchitecture "In computer engineering, computer architecture is a set of rules and methods that describe the functionality, organization, and implementation of computer systems.")
AnnotationAssertion(rdfs:label modsci:ComputerSystemArchitecture "Computer Architecture")
SubClassOf(modsci:ComputerSystemArchitecture modsci:ComputerSoftware)

# Class: modsci:ComputerVision (Computer Vision)

AnnotationAssertion(rdfs:comment modsci:ComputerVision "Computer vision is an interdisciplinary scientific field that deals with how computers can be made to gain high-level understanding from digital images or videos.")
AnnotationAssertion(rdfs:label modsci:ComputerVision "Computer Vision")
SubClassOf(modsci:ComputerVision modsci:ArtificialIntelligence)

# Class: modsci:ConceptualModelling (modsci:ConceptualModelling)

SubClassOf(modsci:ConceptualModelling modsci:InformationSystems)

# Class: modsci:CondensedMatterPhysics (Condensed Matter Physics)

AnnotationAssertion(rdfs:comment modsci:CondensedMatterPhysics "Condensed matter physics is the field of physics that deals with the macroscopic physical properties of matter.")
AnnotationAssertion(rdfs:label modsci:CondensedMatterPhysics "Condensed Matter Physics")
SubClassOf(modsci:CondensedMatterPhysics modsci:Physics)

# Class: modsci:Cosmology (Physical Cosmology)

AnnotationAssertion(rdfs:comment modsci:Cosmology "Physical cosmology is the study of the largest-scale structures and dynamics of the Universe and is concerned with fundamental questions about its origin, structure, evolution, and ultimate fate.")
AnnotationAssertion(rdfs:label modsci:Cosmology "Physical Cosmology")
SubClassOf(modsci:Cosmology modsci:Astronomy)

# Class: modsci:CropProduction (modsci:CropProduction)

SubClassOf(modsci:CropProduction modsci:Agriculture)

# Class: modsci:Cryobiology (Cryobiology)

AnnotationAssertion(rdfs:comment modsci:Cryobiology "Cryobiology is the study of living organisms, organs, biological tissues or biological cells at low temperatures.")
AnnotationAssertion(rdfs:label modsci:Cryobiology "Cryobiology")
SubClassOf(modsci:Cryobiology modsci:Biology)

# Class: modsci:Cryptography (Cryptography)

AnnotationAssertion(rdfs:comment modsci:Cryptography "Cryptography or cryptology is the practice and study of techniques for secure communication in the presence of third parties called adversaries.")
AnnotationAssertion(rdfs:label modsci:Cryptography "Cryptography")
SubClassOf(modsci:Cryptography modsci:CommunicationAndSecurity)

# Class: modsci:Crystallography (Crystallography)

AnnotationAssertion(rdfs:comment modsci:Crystallography "Crystallography is the scientific study of crystals.")
AnnotationAssertion(rdfs:label modsci:Crystallography "Crystallography")
SubClassOf(modsci:Crystallography modsci:Chemistry)

# Class: modsci:CulturalStudies (Cultural Studies)

AnnotationAssertion(rdfs:comment modsci:CulturalStudies "Cultural studies is a field of theoretically, politically, and empirically engaged cultural analysis that concentrates upon the political dynamics of contemporary culture, its historical foundations, defining traits, conflicts, and contingencies.")
AnnotationAssertion(rdfs:label modsci:CulturalStudies "Cultural Studies")
SubClassOf(modsci:CulturalStudies modsci:InterdisciplinaryStudies)

# Class: modsci:Cybernetics (Cybernetics)

AnnotationAssertion(rdfs:comment modsci:Cybernetics "Cybernetics is a transdisciplinary approach for exploring regulatory systems with feedback, their structures, constraints, and possibilities.")
AnnotationAssertion(rdfs:label modsci:Cybernetics "Cybernetics")
SubClassOf(modsci:Cybernetics modsci:InterdisciplinaryStudies)

# Class: modsci:DataEncryption (modsci:DataEncryption)

SubClassOf(modsci:DataEncryption modsci:DataFormat)

# Class: modsci:DataFormat (modsci:DataFormat)

SubClassOf(modsci:DataFormat modsci:ComputerScience)

# Class: modsci:DataMining (Data Mining)

AnnotationAssertion(rdfs:comment modsci:DataMining "Data mining is the process of discovering patterns in large data sets involving methods at the intersection of machine learning, statistics, and database systems.")
AnnotationAssertion(rdfs:label modsci:DataMining "Data Mining")
SubClassOf(modsci:DataMining modsci:DatabaseManagement)

# Class: modsci:DataStructures (modsci:DataStructures)

SubClassOf(modsci:DataStructures modsci:DataFormat)

# Class: modsci:DatabaseManagement (Databases)

AnnotationAssertion(rdfs:comment modsci:DatabaseManagement "Digital databases are managed using database management systems to store, create, maintain, and search data, through database models and query languages.")
AnnotationAssertion(rdfs:label modsci:DatabaseManagement "Databases")
SubClassOf(modsci:DatabaseManagement modsci:InformationSystems)

# Class: modsci:DecisionSupportSystems (modsci:DecisionSupportSystems)

SubClassOf(modsci:DecisionSupportSystems modsci:InformationSystems)

# Class: modsci:Dentistry (Dentistry)

AnnotationAssertion(rdfs:comment modsci:Dentistry "Dentistry, also known as Dental and Oral Medicine, is a branch of medicine that consists of the study, diagnosis, prevention, and treatment of diseases, disorders, and conditions of the oral cavity, commonly in the dentition but also the oral mucosa, and of adjacent and related structures and tissues, particularly in the maxillofacial (jaw and facial) area.")
AnnotationAssertion(rdfs:label modsci:Dentistry "Dentistry")
SubClassOf(modsci:Dentistry modsci:HealthSciences)

# Class: modsci:DevelopmentalBiology (Developmental Biology)

AnnotationAssertion(rdfs:comment modsci:DevelopmentalBiology "Developmental biology is the study of the process by which animals and plants grow and develop.")
AnnotationAssertion(rdfs:label modsci:DevelopmentalBiology "Developmental Biology")
SubClassOf(modsci:DevelopmentalBiology modsci:Biology)

# Class: modsci:DifferentialEquations (modsci:DifferentialEquations)

SubClassOf(modsci:DifferentialEquations modsci:PureMathematics)

# Class: modsci:DiscoveryOfMethods (modsci:DiscoveryOfMethods)

SubClassOf(modsci:DiscoveryOfMethods modsci:ScientificDiscovery)

# Class: modsci:DiscoveryOfPhenomenon (modsci:DiscoveryOfPhenomenon)

SubClassOf(modsci:DiscoveryOfPhenomenon modsci:ScientificDiscovery)

# Class: modsci:DiscreteMathematics (modsci:DiscreteMathematics)

SubClassOf(modsci:DiscreteMathematics modsci:PureMathematics)

# Class: modsci:DistributedComputing (Distributed Computing)

AnnotationAssertion(rdfs:comment modsci:DistributedComputing "Distributed computing is a field of computer science that studies distributed systems. A distributed system is a system whose components are located on different networked computers, which communicate and coordinate their actions by passing messages to one another.")
AnnotationAssertion(rdfs:label modsci:DistributedComputing "Distributed Computing")
SubClassOf(modsci:DistributedComputing modsci:DistributedSystems)

# Class: modsci:DistributedSystems (Concurrent, Parallel, and Distributed systems)

AnnotationAssertion(rdfs:comment modsci:DistributedSystems "Systems in which several computations are executing simultaneously, and potentially interacting with each other.")
AnnotationAssertion(rdfs:label modsci:DistributedSystems "Concurrent, Parallel, and Distributed systems")
SubClassOf(modsci:DistributedSystems modsci:ComputerSoftware)

# Class: modsci:EarthScience (Earth Science)

AnnotationAssertion(rdfs:comment modsci:EarthScience "Earth science (also known as geoscience, the geosciences, or the Earth sciences) includes all the sciences related to the planet Earth.")
AnnotationAssertion(rdfs:label modsci:EarthScience "Earth Science")
SubClassOf(modsci:EarthScience modsci:NaturalScience)

# Class: modsci:EcologicalApplications (modsci:EcologicalApplications)

SubClassOf(modsci:EcologicalApplications modsci:EnvironmentalScience)

# Class: modsci:Ecology (Ecology)

AnnotationAssertion(rdfs:comment modsci:Ecology "Ecology is the branch of science that studies the distribution and interactions between living things and the physical environment.")
AnnotationAssertion(rdfs:label modsci:Ecology "Ecology")
SubClassOf(modsci:Ecology modsci:Biology)
SubClassOf(modsci:Ecology modsci:EarthScience)

# Class: modsci:Economics (Economics)

AnnotationAssertion(rdfs:comment modsci:Economics "Economics is the social science that studies the production, distribution, and consumption of goods and services.")
AnnotationAssertion(rdfs:label modsci:Economics "Economics")
SubClassOf(modsci:Economics modsci:SocialSciences)

# Class: modsci:Education (Education)

AnnotationAssertion(rdfs:comment modsci:Education "Education is the teaching or learning of knowledge, especially to develop the reasoning, judgement and skill required in adult life and professional occupations.")
AnnotationAssertion(rdfs:label modsci:Education "Education")
SubClassOf(modsci:Education modsci:AppliedSciences)

# Class: modsci:ElectroanalyticalChemistry (modsci:ElectroanalyticalChemistry)

SubClassOf(modsci:ElectroanalyticalChemistry modsci:AnalyticalChemistry)

# Class: modsci:Electrochemistry (modsci:Electrochemistry)

SubClassOf(modsci:Electrochemistry modsci:PhysicalChemistry)

# Class: modsci:Electrodynamics (modsci:Electrodynamics)

SubClassOf(modsci:Electrodynamics modsci:ClassicalPhysics)

# Class: modsci:Electrostatics (modsci:Electrostatics)

SubClassOf(modsci:Electrostatics modsci:ClassicalPhysics)

# Class: modsci:Engineering (Engineering)

AnnotationAssertion(rdfs:comment modsci:Engineering "Engineering is the practical application of science. This is accomplished through knowledge, mathematics, and practical experience applied to the design of useful objects or processes.")
AnnotationAssertion(rdfs:label modsci:Engineering "Engineering")
SubClassOf(modsci:Engineering modsci:AppliedSciences)

# Class: modsci:EnvironmentalChemistry (Environmental Chemistry)

AnnotationAssertion(rdfs:comment modsci:EnvironmentalChemistry "Environmental chemistry is the scientific study of the physical, chemical and biochemical properties and processes of polluting substances in the environment.")
AnnotationAssertion(rdfs:label modsci:EnvironmentalChemistry "Environmental Chemistry")
SubClassOf(modsci:EnvironmentalChemistry modsci:Chemistry)

# Class: modsci:EnvironmentalScience (Environmental Science)

AnnotationAssertion(rdfs:comment modsci:EnvironmentalScience "Environmental science is the science of the interactions between the physical, chemical, and biological components of the environment, but with particular attention to the effects of humans on the natural environment.")
AnnotationAssertion(rdfs:label modsci:EnvironmentalScience "Environmental Science")
SubClassOf(modsci:EnvironmentalScience modsci:EarthScience)

# Class: modsci:Epidemiology (Epidemiology)

AnnotationAssertion(rdfs:comment modsci:Epidemiology "Epidemiology is the study and analysis of the distribution (who, when, and where), patterns and determinants of health and disease conditions in defined populations.")
AnnotationAssertion(rdfs:label modsci:Epidemiology "Epidemiology")
SubClassOf(modsci:Epidemiology modsci:HealthSciences)

# Class: modsci:Ergonomics (Ergonomics)

AnnotationAssertion(rdfs:comment modsci:Ergonomics "Human factors and ergonomics is the application of psychological and physiological principles to the (engineering and) design of products, processes, and systems.")
AnnotationAssertion(rdfs:label modsci:Ergonomics "Ergonomics")
SubClassOf(modsci:Ergonomics modsci:AppliedSciences)

# Class: modsci:EthnicStudies (Ethnic Studies)

AnnotationAssertion(rdfs:comment modsci:EthnicStudies "Ethnic studies, in the United States, is the interdisciplinary study of difference—chiefly race, ethnicity, and nation, but also sexuality, gender, and other such markings—and power, as expressed by the state, by civil society, and by individuals.")
AnnotationAssertion(rdfs:label modsci:EthnicStudies "Ethnic Studies")
SubClassOf(modsci:EthnicStudies modsci:InterdisciplinaryStudies)

# Class: modsci:Ethnobiology (Ethnobiology)

AnnotationAssertion(rdfs:comment modsci:Ethnobiology "Ethnobiology is the scientific study of the way living things are treated or used by different human cultures.")
AnnotationAssertion(rdfs:label modsci:Ethnobiology "Ethnobiology")
SubClassOf(modsci:Ethnobiology modsci:Biology)

# Class: modsci:Ethnology (Ethnology)

AnnotationAssertion(rdfs:comment modsci:Ethnology "Ethnology is the science that analyzes human cultures and compares them.")
AnnotationAssertion(rdfs:label modsci:Ethnology "Ethnology")
SubClassOf(modsci:Ethnology modsci:SocialSciences)

# Class: modsci:Ethology (Ethology)

AnnotationAssertion(rdfs:comment modsci:Ethology "Ethology is the scientific and objective study of animal behaviour, usually with a focus on behaviour under natural conditions, and viewing behaviour as an evolutionarily adaptive trait.")
AnnotationAssertion(rdfs:label modsci:Ethology "Ethology")
SubClassOf(modsci:Ethology modsci:BehaviouralSciences)

# Class: modsci:EvolutionaryBiology (Evolutionary Biology)

AnnotationAssertion(rdfs:comment modsci:EvolutionaryBiology "Evolutionary biology is a sub-field of biology concerned with the study of the evolutionary processes that produced the diversity of life on Earth.")
AnnotationAssertion(rdfs:label modsci:EvolutionaryBiology "Evolutionary Biology")
SubClassOf(modsci:EvolutionaryBiology modsci:Biology)

# Class: modsci:EvolutionaryComputation (Evolutionary Computation)

AnnotationAssertion(rdfs:comment modsci:EvolutionaryComputation "In computer science, evolutionary computation is a family of algorithms for global optimization inspired by biological evolution, and the subfield of artificial intelligence and soft computing studying these algorithms.")
AnnotationAssertion(rdfs:label modsci:EvolutionaryComputation "Evolutionary Computation")
SubClassOf(modsci:EvolutionaryComputation modsci:SoftComputing)

# Class: modsci:EvolutionaryPsychology (Evolutionary Psychology)

AnnotationAssertion(rdfs:comment modsci:EvolutionaryPsychology "Evolutionary psychology is a theoretical approach in the social and natural sciences that examines psychological structure from a modern evolutionary perspective.")
AnnotationAssertion(rdfs:label modsci:EvolutionaryPsychology "Evolutionary Psychology")
SubClassOf(modsci:EvolutionaryPsychology modsci:InterdisciplinaryStudies)

# Class: modsci:ExperimentalPhysics (Experimental Physics)

AnnotationAssertion(rdfs:comment modsci:ExperimentalPhysics "Experimental physics is the category of disciplines and sub-disciplines in the field of physics that are concerned with the observation of physical phenomena and experiments.")
AnnotationAssertion(rdfs:label modsci:ExperimentalPhysics "Experimental Physics")
SubClassOf(modsci:ExperimentalPhysics modsci:Physics)

# Class: modsci:ExtragalacticAstronomy (Extragalactic Astronomy)

AnnotationAssertion(rdfs:comment modsci:ExtragalacticAstronomy "It is the study of all astronomical objects which are not covered by galactic astronomy.")
AnnotationAssertion(rdfs:label modsci:ExtragalacticAstronomy "Extragalactic Astronomy")
SubClassOf(modsci:ExtragalacticAstronomy modsci:Astronomy)

# Class: modsci:ExtraterrestrialGeology (modsci:ExtraterrestrialGeology)

SubClassOf(modsci:ExtraterrestrialGeology modsci:Geology)

# Class: modsci:FinancialMathematics (modsci:FinancialMathematics)

SubClassOf(modsci:FinancialMathematics modsci:AppliedMathematics)

# Class: modsci:FisheriesSciences (modsci:FisheriesSciences)

SubClassOf(modsci:FisheriesSciences modsci:Agriculture)

# Class: modsci:FlowAnalysis (modsci:FlowAnalysis)

SubClassOf(modsci:FlowAnalysis modsci:AnalyticalChemistry)

# Class: modsci:FluidPhysics (modsci:FluidPhysics)

SubClassOf(modsci:FluidPhysics modsci:ClassicalPhysics)

# Class: modsci:FoodChemistry (Food Chemistry)

AnnotationAssertion(rdfs:comment modsci:FoodChemistry "Food chemistry is the study of chemical processes and interactions of all biological and non-biological components of foods.")
AnnotationAssertion(rdfs:label modsci:FoodChemistry "Food Chemistry")
SubClassOf(modsci:FoodChemistry modsci:Chemistry)

# Class: modsci:Forensics (Forensics)

AnnotationAssertion(rdfs:comment modsci:Forensics "Forensic science, also known as criminalistics, is the application of science to criminal and civil laws, mainly—on the criminal side—during criminal investigation, as governed by the legal standards of admissible evidence and criminal procedure.")
AnnotationAssertion(rdfs:label modsci:Forensics "Forensics")
SubClassOf(modsci:Forensics modsci:AppliedSciences)

# Class: modsci:Forestry (Forestry)

AnnotationAssertion(rdfs:comment modsci:Forestry "Forestry is the art, science, and practice of studying and managing forests and related natural resources.")
AnnotationAssertion(rdfs:label modsci:Forestry "Forestry")
SubClassOf(modsci:Forestry modsci:Biology)

# Class: modsci:ForestrySciences (modsci:ForestrySciences)

SubClassOf(modsci:ForestrySciences modsci:Agriculture)

# Class: modsci:FormalScience (Formal Science)

AnnotationAssertion(rdfs:comment modsci:FormalScience "Formal sciences are a branch of science studying formal language disciplines concerned with formal systems, such as logic, mathematics, statistics, theoretical computer science, artificial intelligence, information theory, game theory, systems theory, decision theory, and theoretical linguistics.")
AnnotationAssertion(rdfs:label modsci:FormalScience "Formal Science")
SubClassOf(modsci:FormalScience modsci:ModernScience)

# Class: modsci:FreeRadicalChemistry (modsci:FreeRadicalChemistry)

SubClassOf(modsci:FreeRadicalChemistry modsci:OrganicChemistry)

# Class: modsci:FunctionalAnalysis (modsci:FunctionalAnalysis)

SubClassOf(modsci:FunctionalAnalysis modsci:PureMathematics)

# Class: modsci:GalacticAstronomy (Galactic Astronomy)

AnnotationAssertion(rdfs:comment modsci:GalacticAstronomy "The study of everything outside our galaxy, including all other galaxies.")
AnnotationAssertion(rdfs:label modsci:GalacticAstronomy "Galactic Astronomy")
SubClassOf(modsci:GalacticAstronomy modsci:Astronomy)

# Class: modsci:Genetics (Genetics)

AnnotationAssertion(rdfs:comment modsci:Genetics "Genetics is the study of genes, heredity, and the variation of organisms, as well as the medical practice of diagnosing, treating, and counseling patients with genetic disorders.")
AnnotationAssertion(rdfs:label modsci:Genetics "Genetics")
SubClassOf(modsci:Genetics modsci:Biology)

# Class: modsci:Geochemistry (Geochemistry)

AnnotationAssertion(rdfs:comment modsci:Geochemistry "Geochemistry is the science that uses the tools and principles of chemistry to explain the mechanisms behind major geological systems such as the Earth's crust and its oceans.")
AnnotationAssertion(rdfs:label modsci:Geochemistry "Geochemistry")
SubClassOf(modsci:Geochemistry modsci:Chemistry)
SubClassOf(modsci:Geochemistry modsci:Geology)

# Class: modsci:Geochronology (modsci:Geochronology)

SubClassOf(modsci:Geochronology modsci:Geology)

# Class: modsci:Geodesy (Geodesy)

AnnotationAssertion(rdfs:comment modsci:Geodesy "Geodesy is the Earth science of accurately measuring and understanding Earth's geometric shape, orientation in space and gravitational field.")
AnnotationAssertion(rdfs:label modsci:Geodesy "Geodesy")
SubClassOf(modsci:Geodesy modsci:EarthScience)

# Class: modsci:Geodynamics (modsci:Geodynamics)

SubClassOf(modsci:Geodynamics modsci:Geophysics)

# Class: modsci:Geography (Geography)

AnnotationAssertion(rdfs:comment modsci:Geography "Geography is a field of science devoted to the study of the lands, features, inhabitants, and phenomena of the Earth and planets.")
AnnotationAssertion(rdfs:label modsci:Geography "Geography")
SubClassOf(modsci:Geography modsci:EarthScience)

# Class: modsci:GeologicalPhenomena (Geological Phenomena)

AnnotationAssertion(rdfs:comment modsci:GeologicalPhenomena "A geological phenomenon is a phenomenon which is explained by or sheds light on the science of geology.")
AnnotationAssertion(rdfs:label modsci:GeologicalPhenomena "Geological Phenomena")
SubClassOf(modsci:GeologicalPhenomena modsci:NaturalPhenomenon)

# Class: modsci:GeologicalSciences (Geological Sciences)

AnnotationAssertion(rdfs:comment modsci:GeologicalSciences "The Geological Sciences examine the physical and chemical processes within Earth and on its surface, including the study of natural resources and risks to habitable areas.")
AnnotationAssertion(rdfs:label modsci:GeologicalSciences "Geological Sciences")
SubClassOf(modsci:GeologicalSciences modsci:EarthScience)

# Class: modsci:Geology (Geology)

AnnotationAssertion(rdfs:comment modsci:Geology "Geology is an earth science concerned with the solid Earth, the rocks of which it is composed, and the processes by which they change over time.")
AnnotationAssertion(rdfs:label modsci:Geology "Geology")
SubClassOf(modsci:Geology modsci:GeologicalSciences)

# Class: modsci:Geomorphology (Geomorphology)

AnnotationAssertion(rdfs:comment modsci:Geomorphology "Geomorphology is the science of surface features and landforms including the forces and processes that create them.")
AnnotationAssertion(rdfs:label modsci:Geomorphology "Geomorphology")
SubClassOf(modsci:Geomorphology modsci:EarthScience)

# Class: modsci:GeophysicalFluidDynamics (modsci:GeophysicalFluidDynamics)

SubClassOf(modsci:GeophysicalFluidDynamics modsci:Geophysics)

# Class: modsci:Geophysics (Geophysics)

AnnotationAssertion(rdfs:comment modsci:Geophysics "Geophysics the physics of the Earth and its environment in space, and study of earth sciences using quantitative physics methods.")
AnnotationAssertion(rdfs:label modsci:Geophysics "Geophysics")
SubClassOf(modsci:Geophysics modsci:EarthScience)

# Class: modsci:Geothermics (modsci:Geothermics)

SubClassOf(modsci:Geothermics modsci:Geophysics)

# Class: modsci:Gerontology (Gerontology)

AnnotationAssertion(rdfs:comment modsci:Gerontology "Gerontology is the study of the social, cultural, psychological, cognitive, and biological aspects of ageing.")
AnnotationAssertion(rdfs:label modsci:Gerontology "Gerontology")
SubClassOf(modsci:Gerontology modsci:Biology)

# Class: modsci:Glaciology (Glaciology)

AnnotationAssertion(rdfs:comment modsci:Glaciology "Glaciology is the scientific study of glaciers, or more generally ice and natural phenomena that involve ice.")
AnnotationAssertion(rdfs:label modsci:Glaciology "Glaciology")
SubClassOf(modsci:Glaciology modsci:EarthScience)

# Class: modsci:GlobalInformationSystems (modsci:GlobalInformationSystems)

SubClassOf(modsci:GlobalInformationSystems modsci:InformationSystems)

# Class: modsci:Gravimetrics (modsci:Gravimetrics)

SubClassOf(modsci:Gravimetrics modsci:Geophysics)

# Class: modsci:GreenChemistry (Green Chemistry)

AnnotationAssertion(rdfs:comment modsci:GreenChemistry "Green chemistry is the use of chemistry for pollutant source reduction; the definition encompasses therefore all aspects of chemical processes that reduce impact on human health and on the environment.")
AnnotationAssertion(rdfs:label modsci:GreenChemistry "Green Chemistry")
SubClassOf(modsci:GreenChemistry modsci:Chemistry)

# Class: modsci:Health (Health)

AnnotationAssertion(rdfs:comment modsci:Health "Health is a state of physical, mental and social well-being in which disease and infirmity are absent.")
AnnotationAssertion(rdfs:label modsci:Health "Health")
SubClassOf(modsci:Health modsci:InterdisciplinaryStudies)

# Class: modsci:HealthSciences (Health Sciences)

AnnotationAssertion(rdfs:comment modsci:HealthSciences "Health sciences are those sciences which focus on health, or health care, as core parts of their subject matter.")
AnnotationAssertion(rdfs:label modsci:HealthSciences "Health Sciences")
SubClassOf(modsci:HealthSciences modsci:ModernScience)

# Class: modsci:Healthcare (Healthcare)

AnnotationAssertion(rdfs:comment modsci:Healthcare "Healthcare is the maintenance or improvement of health via the prevention, diagnosis, and treatment of disease, illness, injury, and other physical and mental impairments in people.")
AnnotationAssertion(rdfs:label modsci:Healthcare "Healthcare")
SubClassOf(modsci:Healthcare modsci:HealthSciences)

# Class: modsci:History (History of Science)

AnnotationAssertion(rdfs:comment modsci:History "The history of science is the study of the development of science and scientific knowledge, including both the natural and social sciences (the history of the arts and humanities is termed history of scholarship).")
AnnotationAssertion(rdfs:label modsci:History "History of Science")
SubClassOf(modsci:History modsci:FormalScience)

# Class: modsci:HomologicalAlgebra (modsci:HomologicalAlgebra)

SubClassOf(modsci:HomologicalAlgebra modsci:Algebra)

# Class: modsci:HorticulturalProduction (modsci:HorticulturalProduction)

SubClassOf(modsci:HorticulturalProduction modsci:Agriculture)

# Class: modsci:HumanComputerInteraction (Human Computer Interaction)

AnnotationAssertion(rdfs:comment modsci:HumanComputerInteraction "Human–computer interaction (HCI) researches the design and use of computer technology, focused on the interfaces between people (users) and computers. Researchers in the field of HCI observe the ways in which humans interact with computers and design technologies that let humans interact with computers in novel ways.")
AnnotationAssertion(rdfs:label modsci:HumanComputerInteraction "Human Computer Interaction")
SubClassOf(modsci:HumanComputerInteraction modsci:SoftwareEngineering)

# Class: modsci:HumanSciences (Human Sciences)

AnnotationAssertion(rdfs:comment modsci:HumanSciences "Human science is a term applied to the investigation of human life and activities by a rational, systematic and verifiable methodology that acknowledges the validity of both data derived by impartial observation of sensory experience (objective phenomena) and data derived by means of impartial observation of psychological experience (subjective phenomena).")
AnnotationAssertion(rdfs:label modsci:HumanSciences "Human Sciences")
SubClassOf(modsci:HumanSciences modsci:InterdisciplinaryStudies)

# Class: modsci:Hydrology (Hydrology)

AnnotationAssertion(rdfs:comment modsci:Hydrology "Hydrology is the scientific study of the movement, distribution, and quality of water on Earth and other planets, including the water cycle, water resources and environmental watershed sustainability.")
AnnotationAssertion(rdfs:label modsci:Hydrology "Hydrology")
SubClassOf(modsci:Hydrology modsci:EarthScience)

# Class: modsci:ImageProcessing (Image Processing)

AnnotationAssertion(rdfs:comment modsci:ImageProcessing "In computer science, digital image processing is the use of computer algorithms to perform image processing on digital images.")
AnnotationAssertion(rdfs:label modsci:ImageProcessing "Image Processing")
SubClassOf(modsci:ImageProcessing modsci:ComputerScience)

# Class: modsci:Immunology (Immunology)

AnnotationAssertion(rdfs:comment modsci:Immunology "Immunology is the study of the immune system and its reaction to pathogens, as well as its malfunctions (autoimmune diseases, allergies, rejection of organ transplants, immune deficiency).")
AnnotationAssertion(rdfs:label modsci:Immunology "Immunology")
SubClassOf(modsci:Immunology modsci:Biology)

# Class: modsci:IndustrialScience (Industrial Process)

AnnotationAssertion(rdfs:comment modsci:IndustrialScience "An industrial process alters materials or substances.")
AnnotationAssertion(rdfs:label modsci:IndustrialScience "Industrial Process")
SubClassOf(modsci:IndustrialScience modsci:AppliedSciences)

# Class: modsci:Industry (Industry)

AnnotationAssertion(rdfs:comment modsci:Industry "An industry is a sector that produces goods or related services within an economy.")
AnnotationAssertion(rdfs:label modsci:Industry "Industry")

# Class: modsci:InformationRetrieval (modsci:InformationRetrieval)

SubClassOf(modsci:InformationRetrieval modsci:InformationSystems)

# Class: modsci:InformationScience (Information Science)

AnnotationAssertion(rdfs:comment modsci:InformationScience "Information science is a field primarily concerned with the analysis, collection, classification, manipulation, storage, retrieval, movement, dissemination, and protection of information.")
AnnotationAssertion(rdfs:label modsci:InformationScience "Information Science")
SubClassOf(modsci:InformationScience modsci:AppliedSciences)

# Class: modsci:InformationSystems (modsci:InformationSystems)

SubClassOf(modsci:InformationSystems modsci:ComputerScience)

# Class: modsci:InformationSystemsManagement (modsci:InformationSystemsManagement)

SubClassOf(modsci:InformationSystemsManagement modsci:InformationSystems)

# Class: modsci:InformationSystemsTheory (modsci:InformationSystemsTheory)

SubClassOf(modsci:InformationSystemsTheory modsci:InformationSystems)

# Class: modsci:InformationVisualization (Information Visualization)

AnnotationAssertion(rdfs:comment modsci:InformationVisualization "Information visualization or information visualisation is the study of (interactive) visual representations of abstract data to reinforce human cognition.")
AnnotationAssertion(rdfs:label modsci:InformationVisualization "Information Visualization")
SubClassOf(modsci:InformationVisualization modsci:ComputerGraphics)

# Class: modsci:Informetrics (modsci:Informetrics)

SubClassOf(modsci:Informetrics modsci:InformationSystems)

# Class: modsci:InorganicChemistry (Inorganic Chemistry)

AnnotationAssertion(rdfs:comment modsci:InorganicChemistry "Inorganic chemistry is a catch-all discipline that covers everything in chemistry that is not organic chemistry.")
AnnotationAssertion(rdfs:label modsci:InorganicChemistry "Inorganic Chemistry")
SubClassOf(modsci:InorganicChemistry modsci:Chemistry)

# Class: modsci:InorganicGreenChemistry (modsci:InorganicGreenChemistry)

SubClassOf(modsci:InorganicGreenChemistry modsci:InorganicChemistry)

# Class: modsci:Instrument (Instrument)

AnnotationAssertion(rdfs:comment modsci:Instrument "A tool or implement, especially one for precision work."@en)
AnnotationAssertion(rdfs:label modsci:Instrument "Instrument"@en)

# Class: modsci:IntegralEquations (modsci:IntegralEquations)

SubClassOf(modsci:IntegralEquations modsci:ComputationalMathematics)

# Class: modsci:InterdisciplinaryStudies (Interdisciplinary Studies)

AnnotationAssertion(rdfs:comment modsci:InterdisciplinaryStudies "Interdisciplinarity or interdisciplinary studies involves the combining of two or more academic disciplines into one activity (e.g., a research project).")
AnnotationAssertion(rdfs:label modsci:InterdisciplinaryStudies "Interdisciplinary Studies")
SubClassOf(modsci:InterdisciplinaryStudies modsci:ModernScience)

# Class: modsci:InterorganisationalInformationSystems (modsci:InterorganisationalInformationSystems)

SubClassOf(modsci:InterorganisationalInformationSystems modsci:InformationSystems)

# Class: modsci:KnowledgeSystems (modsci:KnowledgeSystems)

SubClassOf(modsci:KnowledgeSystems modsci:InformationSystems)

# Class: modsci:LaboratoryInstrument (Laboratory Instrument)

AnnotationAssertion(rdfs:comment modsci:LaboratoryInstrument "An instrument needed for operations in various laboratories, synthesis and analysis."@en)
AnnotationAssertion(rdfs:label modsci:LaboratoryInstrument "Laboratory Instrument"@en)
EquivalentClasses(modsci:LaboratoryInstrument modsci:ScientificInstrument)
SubClassOf(modsci:LaboratoryInstrument modsci:Instrument)

# Class: modsci:Lasers (modsci:Lasers)

SubClassOf(modsci:Lasers modsci:OpticalPhysics)

# Class: modsci:LibraryScience (Library Science)

AnnotationAssertion(rdfs:comment modsci:LibraryScience "Library science is an interdisciplinary or multidisciplinary field that applies the practices, perspectives, and tools of management, information technology, education, and other areas to libraries; the collection, organization, preservation, and dissemination of information resources; and the political economy of information.")
AnnotationAssertion(rdfs:label modsci:LibraryScience "Library Science")
SubClassOf(modsci:LibraryScience modsci:AppliedSciences)
SubClassOf(modsci:LibraryScience modsci:InterdisciplinaryStudies)

# Class: modsci:Limnology (Limnology)

AnnotationAssertion(rdfs:comment modsci:Limnology "Limnology is a discipline that concerns the study of fresh waters, specifically natural and constructed lakes, ponds, streams, and rivers,")
AnnotationAssertion(rdfs:label modsci:Limnology "Limnology")
SubClassOf(modsci:Limnology modsci:Biology)
SubClassOf(modsci:Limnology modsci:EarthScience)

# Class: modsci:Linguistics (Linguistics)

AnnotationAssertion(rdfs:comment modsci:Linguistics "Linguistics is the scientific study of language.")
AnnotationAssertion(rdfs:label modsci:Linguistics "Linguistics")
SubClassOf(modsci:Linguistics modsci:SocialSciences)

# Class: modsci:Logic (Logic)

AnnotationAssertion(rdfs:comment modsci:Logic "Logic is the study of reasoning, or the study of the principles and criteria of valid inference and demonstration.")
AnnotationAssertion(rdfs:label modsci:Logic "Logic")
SubClassOf(modsci:Logic modsci:InterdisciplinaryStudies)

# Class: modsci:MachineLearning (Machine Learning)

AnnotationAssertion(rdfs:comment modsci:MachineLearning "Machine learning (ML) is the scientific study of algorithms and statistical models that computer systems use to perform a specific task without using explicit instructions, relying on patterns and inference instead.")
AnnotationAssertion(rdfs:label modsci:MachineLearning "Machine Learning")
SubClassOf(modsci:MachineLearning modsci:SoftComputing)

# Class: modsci:Magnetism (modsci:Magnetism)

SubClassOf(modsci:Magnetism modsci:Geophysics)

# Class: modsci:MainGroupMetalChemistry (modsci:MainGroupMetalChemistry)

SubClassOf(modsci:MainGroupMetalChemistry modsci:InorganicChemistry)

# Class: modsci:MarineBiology (Marine Biology)

AnnotationAssertion(rdfs:comment modsci:MarineBiology "Marine biology is the scientific study of organisms that live in the ocean")
AnnotationAssertion(rdfs:label modsci:MarineBiology "Marine Biology")
SubClassOf(modsci:MarineBiology modsci:Biology)

# Class: modsci:MarkupLanguages (modsci:MarkupLanguages)

SubClassOf(modsci:MarkupLanguages modsci:DataFormat)

# Class: modsci:MaterialsChemistry (Materials Science)

AnnotationAssertion(rdfs:comment modsci:MaterialsChemistry "The interdisciplinary field of materials science is the design and discovery of new materials, particularly solids.")
AnnotationAssertion(rdfs:label modsci:MaterialsChemistry "Materials Science")
SubClassOf(modsci:MaterialsChemistry modsci:Chemistry)

# Class: modsci:MathematicalAndTheoreticalBiology (Mathematical and Theoretical Biology)

AnnotationAssertion(rdfs:comment modsci:MathematicalAndTheoreticalBiology "Mathematical and theoretical biology is a branch of biology which employs theoretical analysis, mathematical models and abstractions of the living organisms to investigate the principles that govern the structure, development and behavior of the systems")
AnnotationAssertion(rdfs:label modsci:MathematicalAndTheoreticalBiology "Mathematical and Theoretical Biology")
SubClassOf(modsci:MathematicalAndTheoreticalBiology modsci:Biology)

# Class: modsci:MathematicalLogic (modsci:MathematicalLogic)

SubClassOf(modsci:MathematicalLogic modsci:PureMathematics)

# Class: modsci:MathematicalPhysics (Mathematical Physics)

AnnotationAssertion(rdfs:comment modsci:MathematicalPhysics "Mathematical physics refers to the development of mathematical methods for application to problems in physics.")
AnnotationAssertion(rdfs:label modsci:MathematicalPhysics "Mathematical Physics")
SubClassOf(modsci:MathematicalPhysics modsci:InterdisciplinaryStudies)

# Class: modsci:Mathematics (Mathematics)

AnnotationAssertion(rdfs:comment modsci:Mathematics "Mathematics (colloquially, maths, or math), is the body of knowledge centered on concepts such as quantity, structure, space, and change, and also the academic discipline that studies them.")
AnnotationAssertion(rdfs:label modsci:Mathematics "Mathematics")
SubClassOf(modsci:Mathematics modsci:FormalScience)

# Class: modsci:Measurement (Measurement)

AnnotationAssertion(rdfs:comment modsci:Measurement "Measurement is the assignment of a number to a characteristic of an object or event, which can be compared with other objects or events.")
AnnotationAssertion(rdfs:label modsci:Measurement "Measurement")
SubClassOf(modsci:Measurement modsci:AppliedSciences)

# Class: modsci:Mechanics (Mechanics)

AnnotationAssertion(rdfs:comment modsci:Mechanics "Mechanics is the branch of science concerned with the behavior of physical bodies when subjected to forces or displacements, and the subsequent effects of the bodies on their environment.")
AnnotationAssertion(rdfs:label modsci:Mechanics "Mechanics")
SubClassOf(modsci:Mechanics modsci:Physics)

# Class: modsci:MechanismsOfReactions (modsci:MechanismsOfReactions)

SubClassOf(modsci:MechanismsOfReactions modsci:PhysicalChemistry)

# Class: modsci:MedicinalChemistry (Medicinal Chemistry)

AnnotationAssertion(rdfs:comment modsci:MedicinalChemistry "Medicinal chemistry and pharmaceutical chemistry are disciplines at the intersection of chemistry, especially synthetic organic chemistry, and pharmacology and various other biological specialties, where they are involved with design, chemical synthesis and development for market of pharmaceutical agents, or bio-active molecules (drugs).")
AnnotationAssertion(rdfs:label modsci:MedicinalChemistry "Medicinal Chemistry")
SubClassOf(modsci:MedicinalChemistry modsci:Chemistry)

# Class: modsci:Medicine (Medicine)

AnnotationAssertion(rdfs:comment modsci:Medicine "Medicine is a branch of health science concerned with maintaining human health and restoring it by treating disease and injury; it is both an area of knowledge, a science of body systems and diseases and their treatment, and the applied practice of that knowledge.")
AnnotationAssertion(rdfs:label modsci:Medicine "Medicine")
SubClassOf(modsci:Medicine modsci:HealthSciences)

# Class: modsci:Metabolism (Metabolism)

AnnotationAssertion(rdfs:comment modsci:Metabolism "Metabolism is the set of life-sustaining chemical reactions in organisms.")
AnnotationAssertion(rdfs:label modsci:Metabolism "Metabolism")
SubClassOf(modsci:Metabolism modsci:Biology)

# Class: modsci:Metallurgy (Metallurgy)

AnnotationAssertion(rdfs:comment modsci:Metallurgy "Metallurgy is a domain of materials science and engineering that studies the physical and chemical behavior of metallic elements, their inter-metallic compounds, and their mixtures, which are called alloys.")
AnnotationAssertion(rdfs:label modsci:Metallurgy "Metallurgy")
SubClassOf(modsci:Metallurgy modsci:Chemistry)

# Class: modsci:MetamorphicPetrology (modsci:MetamorphicPetrology)

SubClassOf(modsci:MetamorphicPetrology modsci:Geology)

# Class: modsci:MeteorologicalPhenomena (Meteorological Phenomena)

AnnotationAssertion(rdfs:label modsci:MeteorologicalPhenomena "Meteorological Phenomena")
SubClassOf(modsci:MeteorologicalPhenomena modsci:NaturalPhenomenon)

# Class: modsci:MetrologicalChemistry (modsci:MetrologicalChemistry)

SubClassOf(modsci:MetrologicalChemistry modsci:AnalyticalChemistry)

# Class: modsci:Metrology (Metrology)

AnnotationAssertion(rdfs:comment modsci:Metrology "Metrology is the science of measurement.")
AnnotationAssertion(rdfs:label modsci:Metrology "Metrology")
SubClassOf(modsci:Metrology modsci:AppliedSciences)

# Class: modsci:MilitaryScience (Military Science)

AnnotationAssertion(rdfs:comment modsci:MilitaryScience "Military science is the study of military processes, dentsciitutions, and behavior, along with the study of warfare, and the theory and application of organized coercive force.")
AnnotationAssertion(rdfs:label modsci:MilitaryScience "Military Science")
SubClassOf(modsci:MilitaryScience modsci:AppliedSciences)

# Class: modsci:Mineralogy (modsci:Mineralogy)

SubClassOf(modsci:Mineralogy modsci:Geology)

# Class: modsci:MobileTechnologies (modsci:MobileTechnologies)

SubClassOf(modsci:MobileTechnologies modsci:DistributedSystems)

# Class: modsci:ModernScience (Science)

AnnotationAssertion(rdfs:comment modsci:ModernScience "Science is a systematic enterprise that builds and organizes knowledge in the form of testable explanations and predictions about the universe.")
AnnotationAssertion(rdfs:label modsci:ModernScience "Science")

# Class: modsci:MolecularBiology (Molecular Biology)

AnnotationAssertion(rdfs:comment modsci:MolecularBiology "Molecular biology is the study of biology at a molecular level.")
AnnotationAssertion(rdfs:label modsci:MolecularBiology "Molecular Biology")
SubClassOf(modsci:MolecularBiology modsci:Biology)

# Class: modsci:MolecularPhysics (Molecular Physics)

AnnotationAssertion(rdfs:comment modsci:MolecularPhysics "Molecular physics deals with the physics and chemistry of molecules.")
AnnotationAssertion(rdfs:label modsci:MolecularPhysics "Molecular Physics")
SubClassOf(modsci:MolecularPhysics modsci:Physics)

# Class: modsci:MultimediaProgramming (modsci:MultimediaProgramming)

SubClassOf(modsci:MultimediaProgramming modsci:ComputerSoftware)

# Class: modsci:Museology (Museology)

AnnotationAssertion(rdfs:comment modsci:Museology "Museology or museum studies is the study of museums. It explores the history of museums and their role in society, as well as the activities they engage in, including curating, preservation, public programming, and education.")
AnnotationAssertion(rdfs:label modsci:Museology "Museology")
SubClassOf(modsci:Museology modsci:InterdisciplinaryStudies)

# Class: modsci:Nanochemistry (modsci:Nanochemistry)

SubClassOf(modsci:Nanochemistry modsci:MaterialsChemistry)

# Class: modsci:NaturalLanguageProcessing (Natural language processing (NLP))

AnnotationAssertion(rdfs:comment modsci:NaturalLanguageProcessing "Natural language processing (NLP) is a subfield of linguistics, computer science, information engineering, and artificial intelligence concerned with the interactions between computers and human (natural) languages, in particular how to program computers to process and analyze large amounts of natural language data.")
AnnotationAssertion(rdfs:label modsci:NaturalLanguageProcessing "Natural language processing (NLP)")
SubClassOf(modsci:NaturalLanguageProcessing modsci:ArtificialIntelligence)
SubClassOf(modsci:NaturalLanguageProcessing modsci:ComputerSoftware)
SubClassOf(modsci:NaturalLanguageProcessing modsci:Linguistics)

# Class: modsci:NaturalPhenomenon (Natural Phenomenon)

AnnotationAssertion(rdfs:comment modsci:NaturalPhenomenon "Natural phenomena include gravity, tides, biological processes and oscillation."@en)
AnnotationAssertion(rdfs:label modsci:NaturalPhenomenon "Natural Phenomenon"@en)
SubClassOf(modsci:NaturalPhenomenon sweet:Phenomenon)
DisjointClasses(modsci:NaturalPhenomenon modsci:SocialPhenomenon)

# Class: modsci:NaturalProductsChemistry (modsci:NaturalProductsChemistry)

SubClassOf(modsci:NaturalProductsChemistry modsci:OrganicChemistry)

# Class: modsci:NaturalScience (Natural Sciences)

AnnotationAssertion(rdfs:comment modsci:NaturalScience "The natural sciences are those branches of empirical science that produce a comprehension of the natural world through the use of data collected from it by observation and measurement to construct deterministic and/or stochastic quantitative models of its phenomena.")
AnnotationAssertion(rdfs:label modsci:NaturalScience "Natural Sciences")
SubClassOf(modsci:NaturalScience modsci:ModernScience)

# Class: modsci:Networking (Networking)

AnnotationAssertion(rdfs:comment modsci:Networking "A computer network is a digital telecommunications network which allows nodes to share resources.")
AnnotationAssertion(rdfs:label modsci:Networking "Networking")
SubClassOf(modsci:Networking modsci:CommunicationAndSecurity)

# Class: modsci:NeuralEngineering (Neural Engineering)

AnnotationAssertion(rdfs:comment modsci:NeuralEngineering "Neural engineering is a discipline within biomedical engineering that uses engineering techniques to understand, repair, replace, or enhance neural systems.")
AnnotationAssertion(rdfs:label modsci:NeuralEngineering "Neural Engineering")
SubClassOf(modsci:NeuralEngineering modsci:InterdisciplinaryStudies)

# Class: modsci:Neuroscience (Neuroscience)

AnnotationAssertion(rdfs:comment modsci:Neuroscience "Neuroscience is a field of study which deals with the structure, development, genetics, biochemistry, physiology, pharmacology and pathology of the nervous system.")
AnnotationAssertion(rdfs:label modsci:Neuroscience "Neuroscience")
SubClassOf(modsci:Neuroscience modsci:Biology)
SubClassOf(modsci:Neuroscience modsci:InterdisciplinaryStudies)

# Class: modsci:Non-equilibriumProcesses (modsci:Non-equilibriumProcesses)

SubClassOf(modsci:Non-equilibriumProcesses modsci:PhysicalChemistry)

# Class: modsci:Non-metalChemistry (modsci:Non-metalChemistry)

SubClassOf(modsci:Non-metalChemistry modsci:InorganicChemistry)

# Class: modsci:NonlinearOptics (modsci:NonlinearOptics)

SubClassOf(modsci:NonlinearOptics modsci:OpticalPhysics)

# Class: modsci:NuclearChemistry (Nuclear Chemistry)

AnnotationAssertion(rdfs:comment modsci:NuclearChemistry "Nuclear chemistry is the subfield of chemistry dealing with radioactivity, nuclear processes, and transformations in the nuclei of atoms, such as nuclear transmutation and nuclear properties.")
AnnotationAssertion(rdfs:label modsci:NuclearChemistry "Nuclear Chemistry")
SubClassOf(modsci:NuclearChemistry modsci:Chemistry)

# Class: modsci:NuclearPhysics (modsci:NuclearPhysics)

SubClassOf(modsci:NuclearPhysics modsci:Physics)

# Class: modsci:NumberTheory (modsci:NumberTheory)

SubClassOf(modsci:NumberTheory modsci:PureMathematics)

# Class: modsci:NumericalAnalysis (modsci:NumericalAnalysis)

SubClassOf(modsci:NumericalAnalysis modsci:ComputationalMathematics)

# Class: modsci:Nursing (Nursing)

AnnotationAssertion(rdfs:comment modsci:Nursing "Nursing is a profession within the health care sector focused on the care of individuals, families, and communities so they may attain, maintain, or recover optimal health and quality of life.")
AnnotationAssertion(rdfs:label modsci:Nursing "Nursing")
SubClassOf(modsci:Nursing modsci:HealthSciences)

# Class: modsci:OceanographicPhenomena (Oceanographic Phenomena)

AnnotationAssertion(rdfs:label modsci:OceanographicPhenomena "Oceanographic Phenomena")
SubClassOf(modsci:OceanographicPhenomena modsci:NaturalPhenomenon)

# Class: modsci:Oceanography (Oceanography)

AnnotationAssertion(rdfs:comment modsci:Oceanography "Oceanography also known as oceanology, is the study of the physical and biological aspects of the ocean.")
AnnotationAssertion(rdfs:label modsci:Oceanography "Oceanography")
SubClassOf(modsci:Oceanography modsci:EarthScience)

# Class: modsci:OperatingSystems (Operating Systems)

AnnotationAssertion(rdfs:comment modsci:OperatingSystems "An operating system (OS) is system software that manages computer hardware, software resources, and provides common services for computer programs.")
AnnotationAssertion(rdfs:label modsci:OperatingSystems "Operating Systems")
SubClassOf(modsci:OperatingSystems modsci:ComputerSoftware)

# Class: modsci:OperationsResearch (modsci:OperationsResearch)

SubClassOf(modsci:OperationsResearch modsci:AppliedMathematics)

# Class: modsci:OpticalCommunications (modsci:OpticalCommunications)

SubClassOf(modsci:OpticalCommunications modsci:OpticalPhysics)

# Class: modsci:OpticalPhysics (modsci:OpticalPhysics)

EquivalentClasses(modsci:OpticalPhysics modsci:Optics)
SubClassOf(modsci:OpticalPhysics modsci:Physics)

# Class: modsci:Optics (Optics)

AnnotationAssertion(rdfs:comment modsci:Optics "Optics is the branch of physics that studies the behaviour and properties of light, including its interactions with matter and the construction of instruments that use or detect it.")
AnnotationAssertion(rdfs:label modsci:Optics "Optics")
SubClassOf(modsci:Optics modsci:AppliedSciences)

# Class: modsci:Optimisation (modsci:Optimisation)

SubClassOf(modsci:Optimisation modsci:ComputationalMathematics)

# Class: modsci:Optoelectronics (modsci:Optoelectronics)

SubClassOf(modsci:Optoelectronics modsci:OpticalPhysics)

# Class: modsci:OrdinaryDifferentialEquations (modsci:OrdinaryDifferentialEquations)

SubClassOf(modsci:OrdinaryDifferentialEquations modsci:DifferentialEquations)

# Class: modsci:OreDepositPetrology (modsci:OreDepositPetrology)

SubClassOf(modsci:OreDepositPetrology modsci:Geology)

# Class: modsci:OrganicChemicalSynthesis (modsci:OrganicChemicalSynthesis)

SubClassOf(modsci:OrganicChemicalSynthesis modsci:OrganicChemistry)

# Class: modsci:OrganicChemistry (Organic Chemistry)

AnnotationAssertion(rdfs:comment modsci:OrganicChemistry "Organic chemistry is the study of organic, or carbon based, molecules.")
AnnotationAssertion(rdfs:label modsci:OrganicChemistry "Organic Chemistry")
SubClassOf(modsci:OrganicChemistry modsci:Chemistry)

# Class: modsci:OrganicGreenChemistry (modsci:OrganicGreenChemistry)

SubClassOf(modsci:OrganicGreenChemistry modsci:OrganicChemistry)

# Class: modsci:OrganometallicChemistry (Organometallic Chemistry)

AnnotationAssertion(rdfs:comment modsci:OrganometallicChemistry "Organometallic chemistry is the study of chemical compounds containing bonds between carbon and a metal.")
AnnotationAssertion(rdfs:label modsci:OrganometallicChemistry "Organometallic Chemistry")
SubClassOf(modsci:OrganometallicChemistry modsci:Chemistry)

# Class: modsci:Palaeomagnetism (modsci:Palaeomagnetism)

SubClassOf(modsci:Palaeomagnetism modsci:Geophysics)

# Class: modsci:Palaeontology (modsci:Palaeontology)

SubClassOf(modsci:Palaeontology modsci:Geology)

# Class: modsci:Paleoclimatology (Paleoclimatology)

AnnotationAssertion(rdfs:comment modsci:Paleoclimatology "Paleoclimatology is the study of climates for which systematic measurements were not taken.")
AnnotationAssertion(rdfs:label modsci:Paleoclimatology "Paleoclimatology")
SubClassOf(modsci:Paleoclimatology modsci:EarthScience)

# Class: modsci:Paleontology (Paleontology)

AnnotationAssertion(rdfs:comment modsci:Paleontology "Paleontology is the study of the developing history of life on earth, of ancient plants and animals based on the fossil record, evidence of their existence preserved in rocks.")
AnnotationAssertion(rdfs:label modsci:Paleontology "Paleontology")
SubClassOf(modsci:Paleontology modsci:Biology)

# Class: modsci:Palynology (Palynology)

AnnotationAssertion(rdfs:comment modsci:Palynology "Palynology is literally the \"study of dust\" or of \"particles that are strewn\".")
AnnotationAssertion(rdfs:label modsci:Palynology "Palynology")
SubClassOf(modsci:Palynology modsci:EarthScience)

# Class: modsci:ParallelComputing (Parallel Computing)

AnnotationAssertion(rdfs:comment modsci:ParallelComputing "Parallel computing is a type of computation in which many calculations or the execution of processes are carried out simultaneously.")
AnnotationAssertion(rdfs:label modsci:ParallelComputing "Parallel Computing")
SubClassOf(modsci:ParallelComputing modsci:DistributedSystems)

# Class: modsci:Parasitology (Parasitology)

AnnotationAssertion(rdfs:comment modsci:Parasitology "Parasitology is the study of parasites in host organisms, including humans (medical parasitology).")
AnnotationAssertion(rdfs:label modsci:Parasitology "Parasitology")
SubClassOf(modsci:Parasitology modsci:Biology)

# Class: modsci:PartialDifferentialEquations (modsci:PartialDifferentialEquations)

SubClassOf(modsci:PartialDifferentialEquations modsci:DifferentialEquations)

# Class: modsci:ParticlePhysics (Particle Physics)

AnnotationAssertion(rdfs:comment modsci:ParticlePhysics "Particle physics is a branch of physics that studies the elementary constituents of matter and radiation, and the interactions between them.")
AnnotationAssertion(rdfs:label modsci:ParticlePhysics "Particle Physics")
SubClassOf(modsci:ParticlePhysics modsci:Physics)

# Class: modsci:PastureProduction (modsci:PastureProduction)

SubClassOf(modsci:PastureProduction modsci:Agriculture)

# Class: modsci:PatternRecognition (modsci:PatternRecognition)

SubClassOf(modsci:PatternRecognition modsci:ArtificialIntelligence)

# Class: modsci:PetroleumGeology (modsci:PetroleumGeology)

SubClassOf(modsci:PetroleumGeology modsci:Geology)

# Class: modsci:Pharmacology (Pharmacology)

AnnotationAssertion(rdfs:comment modsci:Pharmacology "Pharmacology is the study of how chemical substances interact with living systems.")
AnnotationAssertion(rdfs:label modsci:Pharmacology "Pharmacology")
SubClassOf(modsci:Pharmacology modsci:Biology)

# Class: modsci:Pharmacy (Pharmacy)

AnnotationAssertion(rdfs:comment modsci:Pharmacy "Pharmacy is the science and technique of preparing, dispensing, and reviewing drugs and providing additional clinical services.")
AnnotationAssertion(rdfs:label modsci:Pharmacy "Pharmacy")
SubClassOf(modsci:Pharmacy modsci:HealthSciences)

# Class: modsci:Philosophy (Philosophy of Science)

AnnotationAssertion(rdfs:comment modsci:Philosophy "Philosophy of science is a branch of philosophy concerned with the foundations, methods, and implications of science.")
AnnotationAssertion(rdfs:label modsci:Philosophy "Philosophy of Science")
SubClassOf(modsci:Philosophy modsci:FormalScience)

# Class: modsci:Photochemistry (Photochemistry)

AnnotationAssertion(rdfs:comment modsci:Photochemistry "Photochemistry, a sub-discipline of chemistry, is the study of the interactions between atoms, small molecules, and light (or electromagnetic radiation).")
AnnotationAssertion(rdfs:label modsci:Photochemistry "Photochemistry")
SubClassOf(modsci:Photochemistry modsci:Chemistry)

# Class: modsci:Photonics (modsci:Photonics)

SubClassOf(modsci:Photonics modsci:OpticalPhysics)

# Class: modsci:Phylogeny (Phylogeny)

AnnotationAssertion(rdfs:comment modsci:Phylogeny "Phylogenetics is the study of the evolutionary history and relationships among individuals or groups of organisms.")
AnnotationAssertion(rdfs:label modsci:Phylogeny "Phylogeny")
SubClassOf(modsci:Phylogeny modsci:Biology)

# Class: modsci:PhysicalChemistry (Physical Chemistry)

AnnotationAssertion(rdfs:comment modsci:PhysicalChemistry "Physical chemistry is the study of macroscopic, atomic, subatomic, and particulate phenomena in chemical systems in terms of the principles, practices, and concepts of physics such as motion, energy, force, time, thermodynamics, quantum chemistry, statistical mechanics, analytical dynamics and chemical equilibrium.")
AnnotationAssertion(rdfs:label modsci:PhysicalChemistry "Physical Chemistry")
SubClassOf(modsci:PhysicalChemistry modsci:Chemistry)

# Class: modsci:PhysicalGeography (Physical Geography)

AnnotationAssertion(rdfs:comment modsci:PhysicalGeography "Physical geography is a subfield of geography, closely related to geology, that focuses on the spatial characteristics of natural processes, within the hydrosphere, biosphere, atmosphere and lithosphere.")
AnnotationAssertion(rdfs:label modsci:PhysicalGeography "Physical Geography")
SubClassOf(modsci:PhysicalGeography modsci:EarthScience)

# Class: modsci:PhysicalOceanography (modsci:PhysicalOceanography)

SubClassOf(modsci:PhysicalOceanography modsci:Oceanography)

# Class: modsci:PhysicalOrganicChemistry (modsci:PhysicalOrganicChemistry)

SubClassOf(modsci:PhysicalOrganicChemistry modsci:OrganicChemistry)

# Class: modsci:PhysicalPhenomena (Physical Phenomena)

AnnotationAssertion(rdfs:label modsci:PhysicalPhenomena "Physical Phenomena")
SubClassOf(modsci:PhysicalPhenomena modsci:NaturalPhenomenon)

# Class: modsci:Physics (Physics)

AnnotationAssertion(rdfs:comment modsci:Physics "Physics is the science of the natural world. It deals with matter, energy, and the fundamental forces that govern the interactions between particles.")
AnnotationAssertion(rdfs:label modsci:Physics "Physics")
SubClassOf(modsci:Physics modsci:NaturalScience)

# Class: modsci:Physiology (Physiology)

AnnotationAssertion(rdfs:comment modsci:Physiology "Physiology is the branch of science that describes the mechanisms of cell, tissue and organ function in organisms.")
AnnotationAssertion(rdfs:label modsci:Physiology "Physiology")
SubClassOf(modsci:Physiology modsci:Biology)

# Class: modsci:PlanetaryScience (Planetary Science)

AnnotationAssertion(rdfs:comment modsci:PlanetaryScience "Planetary science is a broad field of science that studies all planets.")
AnnotationAssertion(rdfs:label modsci:PlanetaryScience "Planetary Science")
SubClassOf(modsci:PlanetaryScience modsci:Astronomy)

# Class: modsci:PlasmaPhysics (Plasma Physics)

AnnotationAssertion(rdfs:comment modsci:PlasmaPhysics "Plasma physics is the study of ionized gases.")
AnnotationAssertion(rdfs:label modsci:PlasmaPhysics "Plasma Physics")
SubClassOf(modsci:PlasmaPhysics modsci:Physics)

# Class: modsci:PoliticalEconomy (Political Economy)

AnnotationAssertion(rdfs:comment modsci:PoliticalEconomy "Political economy is the study of production and trade and their relations with law, custom and government; and with the distribution of national income and wealth.")
AnnotationAssertion(rdfs:label modsci:PoliticalEconomy "Political Economy")
SubClassOf(modsci:PoliticalEconomy modsci:InterdisciplinaryStudies)

# Class: modsci:PoliticalScience (Political Science)

AnnotationAssertion(rdfs:comment modsci:PoliticalScience "Political science is a social science which deals with systems of governance, and the analysis of political activities, political thoughts, and political behavior.")
AnnotationAssertion(rdfs:label modsci:PoliticalScience "Political Science")
SubClassOf(modsci:PoliticalScience modsci:SocialSciences)

# Class: modsci:PolymerisationMechanisms (modsci:PolymerisationMechanisms)

SubClassOf(modsci:PolymerisationMechanisms modsci:MaterialsChemistry)

# Class: modsci:ProgrammingLanguage (Programming Language)

AnnotationAssertion(rdfs:comment modsci:ProgrammingLanguage "A programming language is a formal language, which comprises a set of instructions that produce various kinds of output. Programming languages are used in computer programming to implement algorithms.")
AnnotationAssertion(rdfs:label modsci:ProgrammingLanguage "Programming Language")
SubClassOf(modsci:ProgrammingLanguage modsci:ProgrammingLanguages)

# Class: modsci:ProgrammingLanguageTheory (Programming Language Theory)

AnnotationAssertion(rdfs:comment modsci:ProgrammingLanguageTheory "Programming language theory (PLT) is a branch of computer science that deals with the design, implementation, analysis, characterization, and classification of programming languages and their individual features.")
AnnotationAssertion(rdfs:label modsci:ProgrammingLanguageTheory "Programming Language Theory")
SubClassOf(modsci:ProgrammingLanguageTheory modsci:ProgrammingLanguages)

# Class: modsci:ProgrammingLanguages (Programming Languages and Compilers)

AnnotationAssertion(rdfs:comment modsci:ProgrammingLanguages "Programming languages can be used to accomplish different tasks in different ways.")
AnnotationAssertion(rdfs:label modsci:ProgrammingLanguages "Programming Languages and Compilers")
SubClassOf(modsci:ProgrammingLanguages modsci:ComputerSoftware)

# Class: modsci:Psychology (Psychology)

AnnotationAssertion(rdfs:comment modsci:Psychology "Psychology is a collection of academic, clinical and industrial disciplines concerned with the explanation and prediction of behavior, thinking, emotions, motivations, relationships, potentials and pathologies.")
AnnotationAssertion(rdfs:label modsci:Psychology "Psychology")
SubClassOf(modsci:Psychology modsci:BehaviouralSciences)

# Class: modsci:PureMathematics (modsci:PureMathematics)

SubClassOf(modsci:PureMathematics modsci:Mathematics)

# Class: modsci:QuantumComputing (Quantum Computing)

AnnotationAssertion(rdfs:comment modsci:QuantumComputing "Quantum computing is the use of quantum-mechanical phenomena such as superposition and entanglement to perform computation. A quantum computer is used to perform such computation, which can be implemented theoretically or physically.")
AnnotationAssertion(rdfs:label modsci:QuantumComputing "Quantum Computing")
SubClassOf(modsci:QuantumComputing modsci:TheoryOfComputation)

# Class: modsci:QuantumMechanics (Quantum Mechanics)

AnnotationAssertion(rdfs:comment modsci:QuantumMechanics "Quantum mechanics (also called quantum physics or quantum theory) is a physical theory that is believed to be the formalism underlying the description of all physical systems.")
AnnotationAssertion(rdfs:label modsci:QuantumMechanics "Quantum Mechanics")
SubClassOf(modsci:QuantumMechanics modsci:Physics)

# Class: modsci:QuantumOptics (modsci:QuantumOptics)

SubClassOf(modsci:QuantumOptics modsci:QuantumPhysics)

# Class: modsci:QuantumPhysics (modsci:QuantumPhysics)

SubClassOf(modsci:QuantumPhysics modsci:Physics)

# Class: modsci:Radiobiology (Radiation Biology)

AnnotationAssertion(rdfs:comment modsci:Radiobiology "Radiobiology is a field of clinical and basic medical sciences that involves the study of the action of ionizing radiation on living things, especially health effects of radiation.")
AnnotationAssertion(rdfs:label modsci:Radiobiology "Radiation Biology")
SubClassOf(modsci:Radiobiology modsci:Biology)

# Class: modsci:Radiochemistry (Radiochemistry)

AnnotationAssertion(rdfs:comment modsci:Radiochemistry "Radiochemistry is the chemistry of radioactive materials, where radioactive isotopes of elements are used to study the properties and chemical reactions of non-radioactive isotopes (often within radiochemistry the absence of radioactivity leads to a substance being described as being inactive as the isotopes are stable).")
AnnotationAssertion(rdfs:label modsci:Radiochemistry "Radiochemistry")
SubClassOf(modsci:Radiochemistry modsci:Chemistry)

# Class: modsci:Radiometrics (modsci:Radiometrics)

SubClassOf(modsci:Radiometrics modsci:Geophysics)

# Class: modsci:RelationalDatabases (Relational Databases)

AnnotationAssertion(rdfs:comment modsci:RelationalDatabases "A relational database is a digital database based on the relational model of data, as proposed by E. F. Codd in 1970.")
AnnotationAssertion(rdfs:label modsci:RelationalDatabases "Relational Databases")
SubClassOf(modsci:RelationalDatabases modsci:DatabaseManagement)

# Class: modsci:ReverseEngineering (Reverse Engineering)

AnnotationAssertion(rdfs:comment modsci:ReverseEngineering "Reverse engineering, also called back engineering, is the process by which a man-made object is deconstructed to reveal its designs, architecture, or to extract knowledge from the object; similar to scientific research, the only difference being that scientific research is about a natural phenomenon.")
AnnotationAssertion(rdfs:label modsci:ReverseEngineering "Reverse Engineering")
SubClassOf(modsci:ReverseEngineering modsci:SoftwareEngineering)

# Class: modsci:Robotics (Robotics)

AnnotationAssertion(rdfs:comment modsci:Robotics "Robotics is an interdisciplinary branch of engineering and science that includes mechanical engineering, electronic engineering, information engineering, computer science, and others. Robotics deals with the design, construction, operation, and use of robots, as well as computer systems for their control, sensory feedback, and information processing.")
AnnotationAssertion(rdfs:label modsci:Robotics "Robotics")
SubClassOf(modsci:Robotics modsci:ArtificialIntelligence)

# Class: modsci:ScienceAndTechnologyStudies (Science and Technology Studies)

AnnotationAssertion(rdfs:comment modsci:ScienceAndTechnologyStudies "Science and technology studies is the study of how society, politics, and culture affect scientific research and technological innovation, and how these, in turn, affect society, politics and culture.")
AnnotationAssertion(rdfs:label modsci:ScienceAndTechnologyStudies "Science and Technology Studies")
SubClassOf(modsci:ScienceAndTechnologyStudies modsci:InterdisciplinaryStudies)

# Class: modsci:ScienceStudies (Science Studies)

AnnotationAssertion(rdfs:comment modsci:ScienceStudies "Science studies is an interdisciplinary research area that seeks to situate scientific expertise in broad social, historical, and philosophical contexts.")
AnnotationAssertion(rdfs:label modsci:ScienceStudies "Science Studies")
SubClassOf(modsci:ScienceStudies modsci:InterdisciplinaryStudies)

# Class: modsci:ScientificDiscovery (Scientific Discovery)

AnnotationAssertion(rdfs:comment modsci:ScientificDiscovery "Scientific Discovery is the process or product of successful scientific inquiry. Objects of discovery can be things, events, processes, causes, and properties as well as theories and hypotheses and their features (their explanatory power, for example).")
AnnotationAssertion(rdfs:label modsci:ScientificDiscovery "Scientific Discovery")

# Class: modsci:ScientificInstrument (Scientific Instrument)

AnnotationAssertion(rdfs:comment modsci:ScientificInstrument "A scientific instrument is, broadly speaking, a device or tool used for scientific purposes, including the study of both natural phenomena and theoretical research."@en)
AnnotationAssertion(rdfs:label modsci:ScientificInstrument "Scientific Instrument")
AnnotationAssertion(skos:prefLabel modsci:ScientificInstrument "Instrument"@en)
SubClassOf(modsci:ScientificInstrument modsci:Instrument)

# Class: modsci:ScientificInstrumentManufacturer (Scientific Instrument Manufacturer)

AnnotationAssertion(rdfs:comment modsci:ScientificInstrumentManufacturer "Companies manufacturing equipment for scientific sstudies.")
AnnotationAssertion(rdfs:label modsci:ScientificInstrumentManufacturer "Scientific Instrument Manufacturer")

# Class: modsci:ScientificMethod (Scientific Method)

AnnotationAssertion(rdfs:comment modsci:ScientificMethod "A scientific method is a sequence or collection of processes that are considered characteristic of scientific investigation and the acquisition of new scientific knowledge based upon physical evidence.")
AnnotationAssertion(rdfs:label modsci:ScientificMethod "Scientific Method")

# Class: modsci:ScientificModeling (Scientific Modelling)

AnnotationAssertion(rdfs:comment modsci:ScientificModeling "Scientific modelling is a scientific activity, the aim of which is to make a particular part or feature of the world easier to understand, define, quantify, visualize, or simulate by referencing it to existing and usually commonly accepted knowledge.")
AnnotationAssertion(rdfs:label modsci:ScientificModeling "Scientific Modelling")
SubClassOf(modsci:ScientificModeling modsci:InterdisciplinaryStudies)

# Class: modsci:ScientificOrganization (Scientific Organization)

AnnotationAssertion(rdfs:comment modsci:ScientificOrganization "An organization which is created for the purpose of scientific research and development."@en)
AnnotationAssertion(rdfs:label modsci:ScientificOrganization "Scientific Organization"@en)
SubClassOf(modsci:ScientificOrganization foaf:Organization)

# Class: modsci:Scientist (Scientist)

AnnotationAssertion(rdfs:comment modsci:Scientist "A scientist is someone who conducts scientific research to advance knowledge in an area of interest."@en)
AnnotationAssertion(rdfs:label modsci:Scientist "Scientist"@en)
SubClassOf(modsci:Scientist foaf:Person)

# Class: modsci:Sedimentology (modsci:Sedimentology)

SubClassOf(modsci:Sedimentology modsci:Geology)

# Class: modsci:SeismicExploration (modsci:SeismicExploration)

SubClassOf(modsci:SeismicExploration modsci:Geophysics)

# Class: modsci:Seismology (modsci:Seismology)

SubClassOf(modsci:Seismology modsci:Geophysics)

# Class: modsci:Semantics (Semantics)

AnnotationAssertion(rdfs:comment modsci:Semantics "In programming language theory, semantics is the field concerned with the rigorous mathematical study of the meaning of programming languages. It does so by evaluating the meaning of syntactically valid strings defined by a specific programming language, showing the computation involved.")
AnnotationAssertion(rdfs:label modsci:Semantics "Semantics")
SubClassOf(modsci:Semantics modsci:ProgrammingLanguages)

# Class: modsci:Semiotics (Semiotics)

AnnotationAssertion(rdfs:comment modsci:Semiotics "Semiotics is the study of signs (symbols) and signification systems, or rather semiotics are general theories of signs.")
AnnotationAssertion(rdfs:label modsci:Semiotics "Semiotics")
SubClassOf(modsci:Semiotics modsci:InterdisciplinaryStudies)
SubClassOf(modsci:Semiotics modsci:SocialSciences)

# Class: modsci:SeparationScience (modsci:SeparationScience)

SubClassOf(modsci:SeparationScience modsci:AnalyticalChemistry)

# Class: modsci:SocialPhenomenon (Social Phenomenon)

AnnotationAssertion(rdfs:comment modsci:SocialPhenomenon "Social phenomena are those that occur or exist through the actions of groups of humans."@en)
AnnotationAssertion(rdfs:label modsci:SocialPhenomenon "Social Phenomenon"@en)
SubClassOf(modsci:SocialPhenomenon sweet:Phenomenon)

# Class: modsci:SocialPsychology (Social Psychology)

AnnotationAssertion(rdfs:comment modsci:SocialPsychology "Social psychology is the scientific study of how people's thoughts, feelings, and behaviors are influenced by the actual, imagined or implied presence of others.")
AnnotationAssertion(rdfs:label modsci:SocialPsychology "Social Psychology")
SubClassOf(modsci:SocialPsychology modsci:BehaviouralSciences)

# Class: modsci:SocialSciences (Social Sciences)

AnnotationAssertion(rdfs:comment modsci:SocialSciences "The social sciences are academic disciplines concerned with the study of the social life of human groups and individuals including anthropology, economics, geography, history, political science, psychology, social studies, and sociology.")
AnnotationAssertion(rdfs:label modsci:SocialSciences "Social Sciences")
SubClassOf(modsci:SocialSciences modsci:ModernScience)

# Class: modsci:SocialWork (Social Work)

AnnotationAssertion(rdfs:comment modsci:SocialWork "Social work is an academic discipline and profession that concerns itself with individuals, families, groups and communities in an effort to enhance social functioning and overall well-being.")
AnnotationAssertion(rdfs:label modsci:SocialWork "Social Work")
SubClassOf(modsci:SocialWork modsci:HealthSciences)

# Class: modsci:Sociobiology (Sociobiology)

AnnotationAssertion(rdfs:comment modsci:Sociobiology "Sociobiology is a field of biology that aims to examine and explain social behavior in terms of evolution.")
AnnotationAssertion(rdfs:label modsci:Sociobiology "Sociobiology")
SubClassOf(modsci:Sociobiology modsci:BehaviouralSciences)
SubClassOf(modsci:Sociobiology modsci:Biology)

# Class: modsci:Sociology (Sociology)

AnnotationAssertion(rdfs:comment modsci:Sociology "Sociology is the study of social behaviour or society, including its origins, development, organization, networks, and institutions. and critical analysis to develop a body of knowledge about social order, disorder, and change.")
AnnotationAssertion(rdfs:label modsci:Sociology "Sociology")
SubClassOf(modsci:Sociology modsci:SocialSciences)

# Class: modsci:SoftComputing (Soft Computing)

AnnotationAssertion(rdfs:comment modsci:SoftComputing "Soft computing, as opposed to traditional computing, deals with approximate models and gives solutions to complex real-life problems. Unlike hard computing, soft computing is tolerant of imprecision, uncertainty, partial truth, and approximations.")
AnnotationAssertion(rdfs:label modsci:SoftComputing "Soft Computing")
SubClassOf(modsci:SoftComputing modsci:ArtificialIntelligence)

# Class: modsci:SoftwareEngineering (Software Engineering)

AnnotationAssertion(rdfs:comment modsci:SoftwareEngineering "Software engineering is the application of engineering to the development of software in a systematic method.")
AnnotationAssertion(rdfs:label modsci:SoftwareEngineering "Software Engineering")
SubClassOf(modsci:SoftwareEngineering modsci:ComputerSoftware)

# Class: modsci:SoilBiology (Soil Biology)

AnnotationAssertion(rdfs:comment modsci:SoilBiology "Soil biology is the study of microbial and faunal activity and ecology in soil.")
AnnotationAssertion(rdfs:label modsci:SoilBiology "Soil Biology")
SubClassOf(modsci:SoilBiology modsci:Biology)

# Class: modsci:SoilScience (Soil Science)

AnnotationAssertion(rdfs:comment modsci:SoilScience "Soil science is the study of soil as a natural resource on the surface of the Earth including soil formation, classification and mapping; physical, chemical, biological, and fertility properties of soils; and these properties in relation to the use and management of soils.")
AnnotationAssertion(rdfs:label modsci:SoilScience "Soil Science")
SubClassOf(modsci:SoilScience modsci:EarthScience)

# Class: modsci:SoilSciences (modsci:SoilSciences)

SubClassOf(modsci:SoilSciences modsci:EnvironmentalScience)

# Class: modsci:SolidMechanics (Solid Mechanics)

AnnotationAssertion(rdfs:comment modsci:SolidMechanics "Solid mechanics is a mathematical discipline within continuum mechanics, dealing with the mechanical behavior of solid materials.")
AnnotationAssertion(rdfs:label modsci:SolidMechanics "Solid Mechanics")
SubClassOf(modsci:SolidMechanics modsci:Physics)

# Class: modsci:SolidStateChemistry (Solid-State Chemistry)

AnnotationAssertion(rdfs:comment modsci:SolidStateChemistry "Solid-state chemistry, also sometimes referred as materials chemistry, is the study of the synthesis, structure, and properties of solid phase materials, particularly, but not necessarily exclusively of, non-molecular solids.")
AnnotationAssertion(rdfs:label modsci:SolidStateChemistry "Solid-State Chemistry")
SubClassOf(modsci:SolidStateChemistry modsci:InorganicChemistry)

# Class: modsci:SolutionChemistry (modsci:SolutionChemistry)

SubClassOf(modsci:SolutionChemistry modsci:PhysicalChemistry)

# Class: modsci:SpaceScience (Space Science)

AnnotationAssertion(rdfs:comment modsci:SpaceScience "Space science encompasses all of the scientific disciplines that involve space exploration and study natural phenomena and physical bodies occurring in outer space, such as space medicine and astrobiology.")
AnnotationAssertion(rdfs:label modsci:SpaceScience "Space Science")
SubClassOf(modsci:SpaceScience modsci:EarthScience)

# Class: modsci:Spectroscopy (modsci:Spectroscopy)

SubClassOf(modsci:Spectroscopy modsci:OpticalPhysics)

# Class: modsci:SportsScience (Sports Science)

AnnotationAssertion(rdfs:comment modsci:SportsScience "Sports science is a discipline that studies how the healthy human body works during exercise, and how sport and physical activity promote health and performance from cellular to whole body perspectives.")
AnnotationAssertion(rdfs:label modsci:SportsScience "Sports Science")
SubClassOf(modsci:SportsScience modsci:AppliedSciences)

# Class: modsci:Statistics (Statistics)

AnnotationAssertion(rdfs:comment modsci:Statistics "Statistics is the discipline that concerns the collection, organization, displaying, analysis, interpretation and presentation of data.")
AnnotationAssertion(rdfs:label modsci:Statistics "Statistics")
SubClassOf(modsci:Statistics modsci:FormalScience)

# Class: modsci:StellarAstronomy (Stellar Astronomy)

AnnotationAssertion(rdfs:comment modsci:StellarAstronomy "The study of stars and stellar evolution is fundamental to our understanding of the Universe.")
AnnotationAssertion(rdfs:label modsci:StellarAstronomy "Stellar Astronomy")
SubClassOf(modsci:StellarAstronomy modsci:Astronomy)

# Class: modsci:Stereochemistry (Stereochemistry)

AnnotationAssertion(rdfs:comment modsci:Stereochemistry "Stereochemistry, a subdiscipline of chemistry, involves the study of the relative spatial arrangement of atoms that form the structure of molecules and their manipulation.")
AnnotationAssertion(rdfs:label modsci:Stereochemistry "Stereochemistry")
SubClassOf(modsci:Stereochemistry modsci:Chemistry)

# Class: modsci:Stratigraphy (modsci:Stratigraphy)

SubClassOf(modsci:Stratigraphy modsci:Geology)

# Class: modsci:StructuralChemistry (modsci:StructuralChemistry)

SubClassOf(modsci:StructuralChemistry modsci:PhysicalChemistry)

# Class: modsci:StructuralGeology (modsci:StructuralGeology)

SubClassOf(modsci:StructuralGeology modsci:Geology)

# Class: modsci:StructuredStorage (Structured Storage)

AnnotationAssertion(rdfs:comment modsci:StructuredStorage "Structured storage is computer storage for structured data, often in the form of a distributed database.")
AnnotationAssertion(rdfs:label modsci:StructuredStorage "Structured Storage")
SubClassOf(modsci:StructuredStorage modsci:DatabaseManagement)

# Class: modsci:SupramolecularChemistry (Supramolecular Chemistry)

AnnotationAssertion(rdfs:comment modsci:SupramolecularChemistry "Supramolecular chemistry is a branch of chemistry that describes self-organization or self-assembly of systems to well-defined molecular architectures.")
AnnotationAssertion(rdfs:label modsci:SupramolecularChemistry "Supramolecular Chemistry")
SubClassOf(modsci:SupramolecularChemistry modsci:MaterialsChemistry)

# Class: modsci:SurfaceChemistry (Surface Chemistry)

AnnotationAssertion(rdfs:comment modsci:SurfaceChemistry "Surface chemistry is the study of chemical phenomena that occur at the interface of two phases")
AnnotationAssertion(rdfs:label modsci:SurfaceChemistry "Surface Chemistry")
SubClassOf(modsci:SurfaceChemistry modsci:PhysicalChemistry)

# Class: modsci:SynthesisOfMaterials (modsci:SynthesisOfMaterials)

SubClassOf(modsci:SynthesisOfMaterials modsci:MaterialsChemistry)

# Class: modsci:SystemsScience (Systems Science)

AnnotationAssertion(rdfs:comment modsci:SystemsScience "Systems science is the field of science surrounding systems theory, cybernetics, the science of complex systems.")
AnnotationAssertion(rdfs:label modsci:SystemsScience "Systems Science")
SubClassOf(modsci:SystemsScience modsci:InterdisciplinaryStudies)

# Class: modsci:Technology (Technology)

AnnotationAssertion(rdfs:comment modsci:Technology "Technology is the collection of techniques, skills, methods, and processes used in the production of goods or services or in the accomplishment of objectives, such as scientific investigation.")
AnnotationAssertion(rdfs:label modsci:Technology "Technology")
SubClassOf(modsci:Technology modsci:FormalScience)

# Class: modsci:Tectonics (modsci:Tectonics)

SubClassOf(modsci:Tectonics modsci:Geology)

# Class: modsci:TheoreticalBiology (Theoretical Biology)

AnnotationAssertion(rdfs:comment modsci:TheoreticalBiology "Theoretical biology is a branch of biology which employs theoretical analysis, mathematical models and abstractions of the living organisms to investigate the principles that govern the structure, development and behavior of the systems")
AnnotationAssertion(rdfs:label modsci:TheoreticalBiology "Theoretical Biology")
SubClassOf(modsci:TheoreticalBiology modsci:Biology)

# Class: modsci:TheoreticalChemistry (Theoretical Chemistry)

AnnotationAssertion(rdfs:comment modsci:TheoreticalChemistry "Theoretical chemistry is the application of theoretical reasoning to chemistry.")
AnnotationAssertion(rdfs:label modsci:TheoreticalChemistry "Theoretical Chemistry")
SubClassOf(modsci:TheoreticalChemistry modsci:Chemistry)

# Class: modsci:TheoreticalComputerScience (modsci:TheoreticalComputerScience)

SubClassOf(modsci:TheoreticalComputerScience modsci:ComputerScience)

# Class: modsci:TheoreticalLinguistics (Theoretical Linguistics)

AnnotationAssertion(rdfs:comment modsci:TheoreticalLinguistics "Theoretical linguistics, or general linguistics, is the branch of linguistics which inquires into the nature of language itself and seeks to answer fundamental questions as to what language is; how it works; how universal grammar (UG) as a domain-specific mental organ operates, if it exists at all; what are its unique properties; how does language relate to other cognitive processes, etc.")
AnnotationAssertion(rdfs:label modsci:TheoreticalLinguistics "Theoretical Linguistics")
SubClassOf(modsci:TheoreticalLinguistics modsci:FormalScience)

# Class: modsci:TheoryAndDesignOfMaterials (modsci:TheoryAndDesignOfMaterials)

SubClassOf(modsci:TheoryAndDesignOfMaterials modsci:MaterialsChemistry)

# Class: modsci:TheoryOfComputation (Theory of Computation)

AnnotationAssertion(rdfs:comment modsci:TheoryOfComputation "Theory of computation is focused on answering fundamental questions about what can be computed and what amount of resources are required to perform those computations.")
AnnotationAssertion(rdfs:label modsci:TheoryOfComputation "Theory of Computation")
SubClassOf(modsci:TheoryOfComputation modsci:TheoreticalComputerScience)

# Class: modsci:Thermodynamics (Thermodynamics)

AnnotationAssertion(rdfs:comment modsci:Thermodynamics "Thermodynamics concerns the physics of heat, work, temperature, energy, and entropy.")
AnnotationAssertion(rdfs:label modsci:Thermodynamics "Thermodynamics")
SubClassOf(modsci:Thermodynamics modsci:ClassicalPhysics)

# Class: modsci:Topology (modsci:Topology)

SubClassOf(modsci:Topology modsci:PureMathematics)

# Class: modsci:Toxicology (Toxicology)

AnnotationAssertion(rdfs:comment modsci:Toxicology "Toxicology is a scientific discipline, overlapping with biology, chemistry, pharmacology, and medicine, that involves the study of the adverse effects of chemical substances on living organisms and the practice of diagnosing and treating exposures to toxins and toxicants.")
AnnotationAssertion(rdfs:label modsci:Toxicology "Toxicology")
SubClassOf(modsci:Toxicology modsci:Biology)

# Class: modsci:Transdisciplinarity (Transdisciplinarity)

AnnotationAssertion(rdfs:comment modsci:Transdisciplinarity "Transdisciplinarity connotes a research strategy that crosses many disciplinary boundaries to create a holistic approach.")
AnnotationAssertion(rdfs:label modsci:Transdisciplinarity "Transdisciplinarity")
SubClassOf(modsci:Transdisciplinarity modsci:InterdisciplinaryStudies)

# Class: modsci:TransitionMetalChemistry (modsci:TransitionMetalChemistry)

SubClassOf(modsci:TransitionMetalChemistry modsci:InorganicChemistry)

# Class: modsci:TypeTheory (Type Theory)

AnnotationAssertion(rdfs:comment modsci:TypeTheory "In mathematics, logic, and computer science, a type theory is any of a class of formal systems, some of which can serve as alternatives to set theory as a foundation for all mathematics. In type theory, every \"term\" has a \"type\" and operations are restricted to terms of a certain type.")
AnnotationAssertion(rdfs:label modsci:TypeTheory "Type Theory")
SubClassOf(modsci:TypeTheory modsci:ProgrammingLanguages)

# Class: modsci:UbiquitousComputing (modsci:UbiquitousComputing)

SubClassOf(modsci:UbiquitousComputing modsci:DistributedSystems)

# Class: modsci:UniversalAlgebra (modsci:UniversalAlgebra)

SubClassOf(modsci:UniversalAlgebra modsci:Algebra)

# Class: modsci:UrbanPlanning (Urban Planning)

AnnotationAssertion(rdfs:comment modsci:UrbanPlanning "Urban planning is a technical and political process concerned with the development and design of land use and the built environment, including air, water, and the infrastructure passing into and out of urban areas, such as transportation, communications, and distribution networks.")
AnnotationAssertion(rdfs:label modsci:UrbanPlanning "Urban Planning")
SubClassOf(modsci:UrbanPlanning modsci:InterdisciplinaryStudies)

# Class: modsci:VeterinaryMedicine (Veterinary Medicine)

AnnotationAssertion(rdfs:comment modsci:VeterinaryMedicine "Veterinary medicine is the branch of medicine that deals with the prevention, diagnosis and treatment of disease, disorder and injury in animals.")
AnnotationAssertion(rdfs:label modsci:VeterinaryMedicine "Veterinary Medicine")
SubClassOf(modsci:VeterinaryMedicine modsci:HealthSciences)

# Class: modsci:VeterinarySciences (modsci:VeterinarySciences)

SubClassOf(modsci:VeterinarySciences modsci:Agriculture)

# Class: modsci:VirtualReality (modsci:VirtualReality)

SubClassOf(modsci:VirtualReality modsci:ComputerGraphics)

# Class: modsci:Volcanology (Volcanology)

AnnotationAssertion(rdfs:comment modsci:Volcanology "Volcanology is a branch of geology that deals with the study of volcanoes, lava, magma, and related geological phenomena.")
AnnotationAssertion(rdfs:label modsci:Volcanology "Volcanology")
SubClassOf(modsci:Volcanology modsci:Geology)

# Class: modsci:Waves (modsci:Waves)

SubClassOf(modsci:Waves modsci:ClassicalPhysics)

# Class: modsci:WebSearch (modsci:WebSearch)

SubClassOf(modsci:WebSearch modsci:InformationRetrieval)

# Class: modsci:WebServices (modsci:WebServices)

SubClassOf(modsci:WebServices modsci:InformationSystems)

# Class: modsci:WebTechnologies (modsci:WebTechnologies)

SubClassOf(modsci:WebTechnologies modsci:DistributedSystems)

# Class: modsci:Zoology (Zoology)

AnnotationAssertion(rdfs:comment modsci:Zoology "Zoology is the study of the biology of animals.")
AnnotationAssertion(rdfs:label modsci:Zoology "Zoology")
SubClassOf(modsci:Zoology modsci:Biology)

# Class: modsci:f-BlockChemistry (modsci:f-BlockChemistry)

SubClassOf(modsci:f-BlockChemistry modsci:InorganicChemistry)


############################
#   Named Individuals
############################

# Individual: modsci:ADInstruments (modsci:ADInstruments)

ClassAssertion(modsci:ScientificInstrumentManufacturer modsci:ADInstruments)

# Individual: modsci:Accelerometer (modsci:Accelerometer)

ClassAssertion(modsci:ScientificInstrument modsci:Accelerometer)

# Individual: modsci:Accumulator (modsci:Accumulator)

ClassAssertion(modsci:ScientificInstrument modsci:Accumulator)
ObjectPropertyAssertion(modsci:instrumentInventedBy modsci:Accumulator modsci:Waldemar_Jungner)
DataPropertyAssertion(modsci:InstrumentFunctionDesription modsci:Accumulator "Used to store electrical energy")

# Individual: modsci:AgilentTechnologies (modsci:AgilentTechnologies)

ClassAssertion(modsci:ScientificInstrumentManufacturer modsci:AgilentTechnologies)

# Individual: modsci:Ammeter (modsci:Ammeter)

ClassAssertion(modsci:ScientificInstrument modsci:Ammeter)
ObjectPropertyAssertion(modsci:instrumentInventedBy modsci:Ammeter modsci:Friedrich_Drexler)
DataPropertyAssertion(modsci:InstrumentFunctionDesription modsci:Ammeter "Measure strength of electric current in amperes.")

# Individual: modsci:Anemometer (modsci:Anemometer)

ClassAssertion(modsci:ScientificInstrument modsci:Anemometer)

# Individual: modsci:AntonPaar (modsci:AntonPaar)

ClassAssertion(modsci:ScientificInstrumentManufacturer modsci:AntonPaar)

# Individual: modsci:Astronomical_Studies (modsci:Astronomical_Studies)

ClassAssertion(modsci:Astronomy modsci:Astronomical_Studies)

# Individual: modsci:Aurora (modsci:Aurora)

ClassAssertion(modsci:AtmosphericPhenomena modsci:Aurora)

# Individual: modsci:Barometer (modsci:Barometer)

ClassAssertion(modsci:ScientificInstrument modsci:Barometer)
ObjectPropertyAssertion(modsci:instrumentInventedBy modsci:Barometer modsci:Evangelista_Torricelli)
DataPropertyAssertion(modsci:InstrumentFunctionDesription modsci:Barometer "Used to measure atmospheric pressure and conditions")

# Individual: modsci:Biochip (modsci:Biochip)

ClassAssertion(modsci:ApplicationOfScience modsci:Biochip)
ObjectPropertyAssertion(modsci:isApplicationOfScience modsci:Biochip modsci:Studying_biochemical_reactions)

# Individual: modsci:Biological_Studies (modsci:Biological_Studies)

ClassAssertion(modsci:Biology modsci:Biological_Studies)
ObjectPropertyAssertion(modsci:appliesLawsFrom modsci:Biological_Studies modsci:Physical_Studies)
ObjectPropertyAssertion(modsci:requiresKnowledgeFrom modsci:Biological_Studies modsci:Historical_Studies)

# Individual: modsci:Biomedical_Signals (modsci:Biomedical_Signals)

ClassAssertion(modsci:ScientificDiscovery modsci:Biomedical_Signals)

# Individual: modsci:Biosensors (modsci:Biosensors)

ClassAssertion(modsci:ApplicationOfScience modsci:Biosensors)

# Individual: modsci:Boiling (modsci:Boiling)

ClassAssertion(modsci:PhysicalPhenomena modsci:Boiling)

# Individual: modsci:Breaking_waves (modsci:Breaking_waves)

ClassAssertion(modsci:OceanographicPhenomena modsci:Breaking_waves)

# Individual: modsci:Bruker (modsci:Bruker)

ClassAssertion(modsci:ScientificInstrumentManufacturer modsci:Bruker)

# Individual: modsci:Caliper (modsci:Caliper)

ClassAssertion(modsci:ScientificInstrument modsci:Caliper)

# Individual: modsci:Calorimeter (modsci:Calorimeter)

ClassAssertion(modsci:ScientificInstrument modsci:Calorimeter)

# Individual: modsci:Chemical_Studies (modsci:Chemical_Studies)

ClassAssertion(modsci:Chemistry modsci:Chemical_Studies)
ObjectPropertyAssertion(modsci:hasCloseRelationshipTo modsci:Chemical_Studies modsci:Biological_Studies)
ObjectPropertyAssertion(modsci:hasCloseRelationshipTo modsci:Chemical_Studies modsci:Physical_Studies)

# Individual: modsci:Community_of_European_Solar_Radio_Astronomers (modsci:Community_of_European_Solar_Radio_Astronomers)

ClassAssertion(modsci:ScientificOrganization modsci:Community_of_European_Solar_Radio_Astronomers)

# Individual: modsci:Conservation_of_energy (modsci:Conservation_of_energy)

ClassAssertion(modsci:PhysicalPhenomena modsci:Conservation_of_energy)
ObjectPropertyAssertion(modsci:discoveredByScientist modsci:Conservation_of_energy modsci:Julius_von_Mayer)

# Individual: modsci:Crystal_growth (modsci:Crystal_growth)

ClassAssertion(modsci:PhysicalPhenomena modsci:Crystal_growth)

# Individual: modsci:DNA_Sequencer (modsci:DNA_Sequencer)

ClassAssertion(modsci:ScientificInstrument modsci:DNA_Sequencer)

# Individual: modsci:Decision_Trees (modsci:Decision_Trees)

ClassAssertion(modsci:ClassificationAlgorithms modsci:Decision_Trees)

# Individual: modsci:Decomposition (modsci:Decomposition)

ClassAssertion(modsci:BiologicalPhenomena modsci:Decomposition)

# Individual: modsci:Deep_Learning (modsci:Deep_Learning)

ClassAssertion(modsci:ScientificMethod modsci:Deep_Learning)
ObjectPropertyAssertion(modsci:inspiredFrom modsci:Deep_Learning modsci:Biomedical_Signals)

# Individual: modsci:Dynamo (modsci:Dynamo)

ClassAssertion(modsci:ScientificInstrument modsci:Dynamo)
ObjectPropertyAssertion(modsci:instrumentInventedBy modsci:Dynamo modsci:Michael_Faraday)
DataPropertyAssertion(modsci:InstrumentFunctionDesription modsci:Dynamo "Converts mechanical energy into electrical energy")

# Individual: modsci:Dynamometer (modsci:Dynamometer)

ClassAssertion(modsci:ScientificInstrument modsci:Dynamometer)

# Individual: modsci:E3G (modsci:E3G)

ClassAssertion(modsci:ScientificOrganization modsci:E3G)

# Individual: modsci:EACSL (modsci:EACSL)

ClassAssertion(modsci:ScientificOrganization modsci:EACSL)

# Individual: modsci:Earthquake (modsci:Earthquake)

ClassAssertion(modsci:GeologicalPhenomena modsci:Earthquake)

# Individual: modsci:Economic_Studies (modsci:Economic_Studies)

ClassAssertion(modsci:Economics modsci:Economic_Studies)
ObjectPropertyAssertion(modsci:usesMethodsFrom modsci:Economic_Studies modsci:Statistics_Studies)

# Individual: modsci:Electrometer (modsci:Electrometer)

ClassAssertion(modsci:ScientificInstrument modsci:Electrometer)

# Individual: modsci:Electroscope (modsci:Electroscope)

ClassAssertion(modsci:ScientificInstrument modsci:Electroscope)

# Individual: modsci:Elementar (modsci:Elementar)

ClassAssertion(modsci:ScientificInstrumentManufacturer modsci:Elementar)

# Individual: modsci:Ellipsometer (modsci:Ellipsometer)

ClassAssertion(modsci:ScientificInstrument modsci:Ellipsometer)

# Individual: modsci:Engineering_Studies (modsci:Engineering_Studies)

ClassAssertion(modsci:Engineering modsci:Engineering_Studies)

# Individual: modsci:Erosion (modsci:Erosion)

ClassAssertion(modsci:GeologicalPhenomena modsci:Erosion)

# Individual: modsci:Eudiometer (modsci:Eudiometer)

ClassAssertion(modsci:ScientificInstrument modsci:Eudiometer)

# Individual: modsci:Evangelista_Torricelli (modsci:Evangelista_Torricelli)

ClassAssertion(modsci:Scientist modsci:Evangelista_Torricelli)
ObjectPropertyAssertion(modsci:isStudentOf modsci:Evangelista_Torricelli modsci:Galileo)
ObjectPropertyAssertion(modsci:undertakesResearch modsci:Evangelista_Torricelli modsci:Mathematical_Studies)
ObjectPropertyAssertion(modsci:undertakesResearch modsci:Evangelista_Torricelli modsci:Physical_Studies)

# Individual: modsci:Fire (modsci:Fire)

ClassAssertion(modsci:ChemicalPhenomena modsci:Fire)

# Individual: modsci:Fraunhofer (modsci:Fraunhofer)

ClassAssertion(modsci:ScientificOrganization modsci:Fraunhofer)

# Individual: modsci:Freezing (modsci:Freezing)

ClassAssertion(modsci:PhysicalPhenomena modsci:Freezing)

# Individual: modsci:Friedrich_Drexler (modsci:Friedrich_Drexler)

ClassAssertion(modsci:Scientist modsci:Friedrich_Drexler)
ObjectPropertyAssertion(modsci:undertakesResearch modsci:Friedrich_Drexler modsci:Engineering_Studies)

# Individual: modsci:Galileo (modsci:Galileo)

ClassAssertion(modsci:Scientist modsci:Galileo)

# Individual: modsci:Galvanometer (modsci:Galvanometer)

ClassAssertion(modsci:ScientificInstrument modsci:Galvanometer)
ObjectPropertyAssertion(modsci:instrumentInventedBy modsci:Galvanometer modsci:Johann_Schweigger)
DataPropertyAssertion(modsci:InstrumentFunctionDesription modsci:Galvanometer "Used to reproduce the recorded sound")

# Individual: modsci:Genetic_algorithms (modsci:Genetic_algorithms)

ClassAssertion(modsci:ScientificMethod modsci:Genetic_algorithms)

# Individual: modsci:Geological_Studies (modsci:Geological_Studies)

ClassAssertion(modsci:Geology modsci:Geological_Studies)

# Individual: modsci:Gravitometer (modsci:Gravitometer)

ClassAssertion(modsci:ScientificInstrument modsci:Gravitometer)

# Individual: modsci:Gravity (modsci:Gravity)

ClassAssertion(modsci:PhysicalPhenomena modsci:Gravity)
ObjectPropertyAssertion(modsci:discoveredByScientist modsci:Gravity modsci:Isaac_Newton)

# Individual: modsci:Growth (modsci:Growth)

ClassAssertion(modsci:BiologicalPhenomena modsci:Growth)

# Individual: modsci:Guglielmo_Marconi (modsci:Guglielmo_Marconi)

ClassAssertion(modsci:Scientist modsci:Guglielmo_Marconi)
ObjectPropertyAssertion(modsci:undertakesResearch modsci:Guglielmo_Marconi modsci:Engineering_Studies)
ObjectPropertyAssertion(modsci:undertakesResearch modsci:Guglielmo_Marconi modsci:Physical_Studies)

# Individual: modsci:Haze (modsci:Haze)

ClassAssertion(modsci:AtmosphericPhenomena modsci:Haze)

# Individual: modsci:Historical_Studies (modsci:Historical_Studies)

ClassAssertion(modsci:History modsci:Historical_Studies)

# Individual: modsci:Horiba (modsci:Horiba)

ClassAssertion(modsci:ScientificInstrumentManufacturer modsci:Horiba)

# Individual: modsci:Hydrometer (modsci:Hydrometer)

ClassAssertion(modsci:ScientificInstrument modsci:Hydrometer)

# Individual: modsci:Inclinometer (modsci:Inclinometer)

ClassAssertion(modsci:ScientificInstrument modsci:Inclinometer)

# Individual: modsci:Interferometer (modsci:Interferometer)

ClassAssertion(modsci:ScientificInstrument modsci:Interferometer)

# Individual: modsci:Isaac_Newton (modsci:Isaac_Newton)

ClassAssertion(modsci:Scientist modsci:Isaac_Newton)
ObjectPropertyAssertion(modsci:undertakesResearch modsci:Isaac_Newton modsci:Astronomical_Studies)
ObjectPropertyAssertion(modsci:undertakesResearch modsci:Isaac_Newton modsci:Mathematical_Studies)
ObjectPropertyAssertion(modsci:undertakesResearch modsci:Isaac_Newton modsci:Physical_Studies)

# Individual: modsci:Johann_Schweigger (modsci:Johann_Schweigger)

ClassAssertion(modsci:Scientist modsci:Johann_Schweigger)
ObjectPropertyAssertion(modsci:undertakesResearch modsci:Johann_Schweigger modsci:Chemical_Studies)
ObjectPropertyAssertion(modsci:undertakesResearch modsci:Johann_Schweigger modsci:Mathematical_Studies)
ObjectPropertyAssertion(modsci:undertakesResearch modsci:Johann_Schweigger modsci:Physical_Studies)

# Individual: modsci:Julius_von_Mayer (modsci:Julius_von_Mayer)

ClassAssertion(modsci:Scientist modsci:Julius_von_Mayer)
ObjectPropertyAssertion(modsci:undertakesResearch modsci:Julius_von_Mayer modsci:Chemical_Studies)
ObjectPropertyAssertion(modsci:undertakesResearch modsci:Julius_von_Mayer modsci:Physical_Studies)

# Individual: modsci:KNN_Algorithm (modsci:KNN_Algorithm)

ClassAssertion(modsci:ClassificationAlgorithms modsci:KNN_Algorithm)

# Individual: modsci:LECO_Corporation (modsci:LECO_Corporation)

ClassAssertion(modsci:ScientificInstrumentManufacturer modsci:LECO_Corporation)

# Individual: modsci:Light_Bulb (modsci:Light_Bulb)

ClassAssertion(modsci:ScientificDiscovery modsci:Light_Bulb)
ObjectPropertyAssertion(modsci:instrumentInventedBy modsci:Light_Bulb modsci:Thomas_Edison)

# Individual: modsci:Light_magnification (modsci:Light_magnification)

ClassAssertion(modsci:Astronomy modsci:Light_magnification)

# Individual: modsci:Light_pillar (modsci:Light_pillar)

ClassAssertion(modsci:AtmosphericPhenomena modsci:Light_pillar)

# Individual: modsci:Linear_Regression (modsci:Linear_Regression)

ClassAssertion(modsci:Statistics modsci:Linear_Regression)

# Individual: modsci:Magnetograph (modsci:Magnetograph)

ClassAssertion(modsci:ScientificInstrument modsci:Magnetograph)

# Individual: modsci:Magnetometer (modsci:Magnetometer)

ClassAssertion(modsci:ScientificInstrument modsci:Magnetometer)

# Individual: modsci:MalvernInstruments (modsci:MalvernInstruments)

ClassAssertion(modsci:ScientificInstrumentManufacturer modsci:MalvernInstruments)

# Individual: modsci:Manometer (modsci:Manometer)

ClassAssertion(modsci:ScientificInstrument modsci:Manometer)

# Individual: modsci:MarkesInternational (modsci:MarkesInternational)

ClassAssertion(modsci:ScientificInstrumentManufacturer modsci:MarkesInternational)

# Individual: modsci:Mathematical_Studies (modsci:Mathematical_Studies)

ClassAssertion(modsci:Mathematics modsci:Mathematical_Studies)
ObjectPropertyAssertion(modsci:requiresKnowledgeFrom modsci:Mathematical_Studies modsci:Mathematical_Studies)

# Individual: modsci:McPhersonInc (modsci:McPhersonInc)

ClassAssertion(modsci:ScientificInstrumentManufacturer modsci:McPhersonInc)

# Individual: modsci:Metabolism (Metabolism)

ClassAssertion(modsci:BiologicalPhenomena modsci:Metabolism)

# Individual: modsci:Michael_Faraday (modsci:Michael_Faraday)

ClassAssertion(modsci:Scientist modsci:Michael_Faraday)
ObjectPropertyAssertion(modsci:undertakesResearch modsci:Michael_Faraday modsci:Chemical_Studies)

# Individual: modsci:Micrometer (modsci:Micrometer)

ClassAssertion(modsci:ScientificInstrument modsci:Micrometer)

# Individual: modsci:Microscope (modsci:Microscope)

ClassAssertion(modsci:ScientificInstrument modsci:Microscope)

# Individual: modsci:Movie_camera (modsci:Movie_camera)

ClassAssertion(modsci:ScientificDiscovery modsci:Movie_camera)
ObjectPropertyAssertion(modsci:instrumentInventedBy modsci:Movie_camera modsci:Thomas_Edison)
DataPropertyAssertion(modsci:InstrumentFunctionDesription modsci:Movie_camera "take a rapid sequence of photographs on an image sensor or on a film.")

# Individual: modsci:NASA (modsci:NASA)

ClassAssertion(modsci:ScientificOrganization modsci:NASA)

# Individual: modsci:NovacamTechnologies (modsci:NovacamTechnologies)

ClassAssertion(modsci:ScientificInstrumentManufacturer modsci:NovacamTechnologies)

# Individual: modsci:Ocean_currents (modsci:Ocean_currents)

ClassAssertion(modsci:OceanographicPhenomena modsci:Ocean_currents)

# Individual: modsci:Ohmmeter (modsci:Ohmmeter)

ClassAssertion(modsci:ScientificInstrument modsci:Ohmmeter)

# Individual: modsci:Olaus_Roemer (modsci:Olaus_Roemer)

ClassAssertion(modsci:Scientist modsci:Olaus_Roemer)
ObjectPropertyAssertion(modsci:undertakesResearch modsci:Olaus_Roemer modsci:Astronomical_Studies)

# Individual: modsci:OpenAI_Inc (modsci:OpenAI_Inc)

ClassAssertion(modsci:ScientificOrganization modsci:OpenAI_Inc)

# Individual: modsci:Oscilloscope (modsci:Oscilloscope)

ClassAssertion(modsci:ScientificInstrument modsci:Oscilloscope)

# Individual: modsci:Overpopulation (modsci:Overpopulation)

ClassAssertion(modsci:BiologicalPhenomena modsci:Overpopulation)

# Individual: modsci:OxfordInstruments (modsci:OxfordInstruments)

ClassAssertion(modsci:ScientificInstrumentManufacturer modsci:OxfordInstruments)

# Individual: modsci:PallCorp (modsci:PallCorp)

ClassAssertion(modsci:ScientificInstrumentManufacturer modsci:PallCorp)

# Individual: modsci:Phonograph (modsci:Phonograph)

ClassAssertion(modsci:ScientificInstrument modsci:Phonograph)
ObjectPropertyAssertion(modsci:instrumentInventedBy modsci:Phonograph modsci:Thomas_Edison)
DataPropertyAssertion(modsci:InstrumentFunctionDesription modsci:Phonograph "record the mechanical and reproduction of sound.")

# Individual: modsci:Physical_Studies (modsci:Physical_Studies)

ClassAssertion(modsci:Physics modsci:Physical_Studies)

# Individual: modsci:PolymerChar (modsci:PolymerChar)

ClassAssertion(modsci:ScientificInstrumentManufacturer modsci:PolymerChar)

# Individual: modsci:Population_decrease (modsci:Population_decrease)

ClassAssertion(modsci:BiologicalPhenomena modsci:Population_decrease)

# Individual: modsci:PsychiatricDrugs (modsci:PsychiatricDrugs)

ClassAssertion(modsci:ApplicationOfScience modsci:PsychiatricDrugs)

# Individual: modsci:Psychological_Studies (modsci:Psychological_Studies)

ClassAssertion(modsci:Psychology modsci:Psychological_Studies)

# Individual: modsci:Racism (modsci:Racism)

ClassAssertion(modsci:SocialPhenomenon modsci:Racism)

# Individual: modsci:Radio_Signals (modsci:Radio_Signals)

ClassAssertion(sweet:Phenomenon modsci:Radio_Signals)
ObjectPropertyAssertion(modsci:discoveredByScientist modsci:Radio_Signals modsci:Guglielmo_Marconi)

# Individual: modsci:Rainbow (modsci:Rainbow)

ClassAssertion(modsci:AtmosphericPhenomena modsci:Rainbow)

# Individual: modsci:Resampling_Methods (modsci:Resampling_Methods)

ClassAssertion(modsci:Statistics modsci:Resampling_Methods)

# Individual: modsci:Rusting (modsci:Rusting)

ClassAssertion(modsci:ChemicalPhenomena modsci:Rusting)

# Individual: modsci:Seismometer (modsci:Seismometer)

ClassAssertion(modsci:ScientificInstrument modsci:Seismometer)

# Individual: modsci:ShimadzuCorp (modsci:ShimadzuCorp)

ClassAssertion(modsci:ScientificInstrumentManufacturer modsci:ShimadzuCorp)

# Individual: modsci:Shrinkage (modsci:Shrinkage)

ClassAssertion(modsci:Statistics modsci:Shrinkage)

# Individual: modsci:Spectrogram (modsci:Spectrogram)

ClassAssertion(modsci:ScientificInstrument modsci:Spectrogram)

# Individual: modsci:Spectrometer (modsci:Spectrometer)

ClassAssertion(modsci:ScientificInstrument modsci:Spectrometer)

# Individual: modsci:Speed_of_light (modsci:Speed_of_light)

ClassAssertion(modsci:ScientificDiscovery modsci:Speed_of_light)
ObjectPropertyAssertion(modsci:discoveredByScientist modsci:Speed_of_light modsci:Olaus_Roemer)

# Individual: modsci:Statistics_Studies (modsci:Statistics_Studies)

ClassAssertion(modsci:Statistics modsci:Statistics_Studies)

# Individual: modsci:Storm (modsci:Storm)

ClassAssertion(modsci:MeteorologicalPhenomena modsci:Storm)

# Individual: modsci:Studying_biochemical_reactions (modsci:Studying_biochemical_reactions)

ClassAssertion(modsci:MolecularBiology modsci:Studying_biochemical_reactions)

# Individual: modsci:Subset_Selection (modsci:Subset_Selection)

ClassAssertion(modsci:Statistics modsci:Subset_Selection)

# Individual: modsci:Subsun (modsci:Subsun)

ClassAssertion(modsci:AtmosphericPhenomena modsci:Subsun)

# Individual: modsci:Supernova (modsci:Supernova)

ClassAssertion(modsci:AstronomicalPhenomena modsci:Supernova)

# Individual: modsci:Support_Vector_Machines (modsci:Support_Vector_Machines)

ClassAssertion(modsci:ClassificationAlgorithms modsci:Support_Vector_Machines)

# Individual: modsci:Techtron (modsci:Techtron)

ClassAssertion(modsci:ScientificInstrumentManufacturer modsci:Techtron)

# Individual: modsci:Telescope (modsci:Telescope)

ClassAssertion(modsci:ScientificInstrument modsci:Telescope)
ObjectPropertyAssertion(modsci:instrumentUsedInScience modsci:Telescope modsci:Light_magnification)

# Individual: modsci:The_Bridges_Organization (modsci:The_Bridges_Organization)

ClassAssertion(modsci:ScientificOrganization modsci:The_Bridges_Organization)

# Individual: modsci:The_Fibonacci_Association (modsci:The_Fibonacci_Association)

ClassAssertion(modsci:ScientificOrganization modsci:The_Fibonacci_Association)

# Individual: modsci:Theodolite (modsci:Theodolite)

ClassAssertion(modsci:ScientificInstrument modsci:Theodolite)

# Individual: modsci:Thermocouple (modsci:Thermocouple)

ClassAssertion(modsci:ScientificInstrument modsci:Thermocouple)

# Individual: modsci:Thermometer (modsci:Thermometer)

ClassAssertion(modsci:ScientificInstrument modsci:Thermometer)
ObjectPropertyAssertion(modsci:instrumentUsedInScience modsci:Thermometer modsci:Studying_biochemical_reactions)
DataPropertyAssertion(modsci:InstrumentFunctionDesription modsci:Thermometer "measure temperature or a temperature gradient.")

# Individual: modsci:Thomas_Edison (modsci:Thomas_Edison)

AnnotationAssertion(foaf:familyName modsci:Thomas_Edison "Edison")
ClassAssertion(modsci:Scientist modsci:Thomas_Edison)

# Individual: modsci:Time_Series_Analysis (modsci:Time_Series_Analysis)

ClassAssertion(modsci:Statistics modsci:Time_Series_Analysis)

# Individual: modsci:Tsunamis (modsci:Tsunamis)

ClassAssertion(modsci:OceanographicPhenomena modsci:Tsunamis)

# Individual: modsci:Volcano (modsci:Volcano)

ClassAssertion(modsci:GeologicalPhenomena modsci:Volcano)

# Individual: modsci:Voltmeter (modsci:Voltmeter)

ClassAssertion(modsci:ScientificInstrument modsci:Voltmeter)

# Individual: modsci:Waldemar_Jungner (modsci:Waldemar_Jungner)

ClassAssertion(modsci:Scientist modsci:Waldemar_Jungner)

# Individual: modsci:WatersCorporation (modsci:WatersCorporation)

ClassAssertion(modsci:ScientificInstrumentManufacturer modsci:WatersCorporation)

# Individual: modsci:Weddings (modsci:Weddings)

ClassAssertion(modsci:SocialPhenomenon modsci:Weddings)

# Individual: modsci:study_of_wetlands (modsci:study_of_wetlands)

ClassAssertion(modsci:Ecology modsci:study_of_wetlands)

# Individual: modsci:temperature_gradient (modsci:temperature_gradient)

ClassAssertion(modsci:PhysicalPhenomena modsci:temperature_gradient)


DLSafeRule(Annotation(<http://swrl.stanford.edu/ontologies/3.3/swrla.owl#isRuleEnabled> "true"^^xsd:boolean) Annotation(rdfs:comment ""^^xsd:string) Annotation(rdfs:label "S3"^^xsd:string) Body(ObjectPropertyAtom(modsci:isDiscoveredBy Variable(modsci:y) Variable(modsci:x)) ClassAtom(modsci:ScientificOrganization Variable(modsci:x)))Head(ObjectPropertyAtom(modsci:isDiscoveredByOrganization Variable(modsci:y) Variable(modsci:x))))
DLSafeRule(Annotation(<http://swrl.stanford.edu/ontologies/3.3/swrla.owl#isRuleEnabled> "true"^^xsd:boolean) Annotation(rdfs:comment ""^^xsd:string) Annotation(rdfs:label "S2"^^xsd:string) Body(ObjectPropertyAtom(modsci:isDiscoveredBy Variable(modsci:y) Variable(modsci:x)) ClassAtom(modsci:Scientist Variable(modsci:x)))Head(ObjectPropertyAtom(modsci:isDiscoveredByScientist Variable(modsci:y) Variable(modsci:x))))
DLSafeRule(Annotation(<http://swrl.stanford.edu/ontologies/3.3/swrla.owl#isRuleEnabled> "true"^^xsd:boolean) Annotation(rdfs:comment ""^^xsd:string) Annotation(rdfs:label "S1"^^xsd:string) Body(ObjectPropertyAtom(modsci:discoveredByScience Variable(modsci:x) Variable(modsci:z)) ObjectPropertyAtom(modsci:discoveredByScientist Variable(modsci:x) Variable(modsci:y)))Head(ObjectPropertyAtom(modsci:scientistBelongsTo Variable(modsci:y) Variable(modsci:z))))
)
